@prefix : <https://ontology.golemlab.eu/> .
@prefix dc: <http://purl.org/dc/elements/1.1/> .
@prefix gc: <https://ontology.golemlab.eu/> .
@prefix dlp: <http://www.ontologydesignpatterns.org/ont/dlp/> .
@prefix owl: <http://www.w3.org/2002/07/owl#> .
@prefix rdf: <http://www.w3.org/1999/02/22-rdf-syntax-ns#> .
@prefix xml: <http://www.w3.org/XML/1998/namespace> .
@prefix xsd: <http://www.w3.org/2001/XMLSchema#> .
@prefix rdfs: <http://www.w3.org/2000/01/rdf-schema#> .
@prefix skos: <http://www.w3.org/2004/02/skos/core#> .
@prefix golem: <https://golemlab.eu/graph/> .
@base <https://ontology.golemlab.eu/> .

<https://ontology.golemlab.eu/> rdf:type owl:Ontology ;
                                 dc:title "GOLEM Ontology" ;
                                 rdfs:comment """# Golem Ontology for Narrative and Fiction

### GOLEM v1.0

Created by [GOLEM lab](https://golemlab.eu/), October 10, 2024

[CC BY 4.0](https://creativecommons.org/licenses/by/4.0/legalcode)

### Overview

Ontology of fiction and narrative, developed as an extension of [CIDOC-CRM](https://cidoc-crm.org/versions-of-the-cidoc-crm) and [LRMoo](https://cidoc-crm.org/frbroo/fm_releases), and aligned to [DOLCE-Lite-Plus](https://www.w3.org/2001/sw/BestPractices/WNET/DLP3941_daml.html).

Narrative phenomena can be viewed as interconnected systems in which various components influence one another. Understanding the properties of narratives requires analyzing them in relation to each other and within their broader context, rather than in isolation ([Pianzola, 2018](https://golemlab.eu/publications/complexity/)). Formal ontologies provide a structured and systematic approach to representing the essential elements of storytelling. By capturing relevant concepts, constraints, and interrelationships among narrative elements, ontology ensures a consistent and explicit representation of the narrative domain.

In literary studies, traditional quantitative and probabilistic methods often struggle to account for the semantic richness and intensional qualities of texts ([Ciotti, 2016](https://impactum-journals.uc.pt/matlit/article/download/2182-8830_4-1_2/1932?inline=1)). In contrast, ontology modeling highlights the complexities of narrative structure, making these elements explicit and computable.

The GOLEM project developed an ontology that models narratives and fiction independently of their specific domains. To achieve this, the project seeks to identify a common ground that defines how key elements of narrative structure—such as events, characters, social relationships, and settings—interrelate. By employing a modularization approach, GOLEM will create a comprehensive library of modules that encapsulate these narrative components, including modules for characters, relationships, events, settings, and narrative inference.

The detailed description of each module can be read in the [GitHub](https://github.com/GOLEM-lab/golem-ontology/wiki).

Furthermore, the ontology contributes to comparative studies by providing a structured framework for analyzing narratives across different cultural contexts. It enhances our understanding of cumulative cultural evolution in narratives, allowing for a more nuanced exploration of how narratives evolve and grows cumulatively over time ([Pianzola et al., 2020](https://ceur-ws.org/Vol-2723/short8.pdf)).

### References

Abbott, H. P. (2019). Narrativity. In P. Hühn et al. (Eds.), *The living handbook of narratology*. Hamburg University.

Bartalesi, V., Meghini, C., & Metilli, D. (2017). A conceptualisation of narratives and its expression in the CRM. *International Journal of Metadata, Semantics and Ontologies*, 12(1), 35-46. https://doi.org/10.1504/IJMSO.2017.10005083

Bekiari, C., Bruseker, G., Canning, E., Doerr, M., Michon, P., Ore, C.-E., Stead, S., & Velios, A. (2024, October). Conceptual reference model (CIDOC CRM), version 7.3 (Tech. rep.). CIDOC CRM-SIG.

Carroll, N. (2015). Interpretation. In *The Routledge companion to philosophy of literature* (pp. 302–312). Routledge.

Chaturvedi, S., Srivastava, S., Daume III, H., & Dyer, C. (2015). Modeling dynamic relationships between characters in literary novels. *arXiv preprint arXiv:1511.09376*. http://arxiv.org/abs/1511.09376

Ciotti, F. (2016). Toward a formal ontology for narrative. *MATLIT: Materialidades da Literatura*, 4(1), 29-44.

Doerr, M., Kritsotaki, A., Rousakis, Y., Hiebel, G., & Theodoridou, M. (2023, October). CRMsci: The scientific observation model (Tech. rep.). CIDOC CRM-SIG.

Jannidis, F. (2019). Character. In P. Hühn et al. (Eds.), *The living handbook of narratology*. Hamburg University.

Kukkonen, K. (2019). Plot. In P. Hühn et al. (Eds.), *The living handbook of narratology*. Hamburg University.

Lea, K. M. (1962). *Italian popular comedy: A study in the commedia dell'arte, 1560–1620 with special reference to the English stage* (Vol. 1). Russell & Russell.

Mika, P., & Gangemi, A. (2016). Descriptions of social relations. *Benefits*, 1, 14. https://doi.org/10.3390/benefits1010014

Pannach, F. (2023, July). “Orpheus came to his end by being struck by a thunderbolt”: Annotating events in mythological sequences. In *Proceedings of the 17th Linguistic Annotation Workshop (LAW-XVII)* (pp. 10-18).

Pannach, F. A. K. (2024). Narrative echoes across time and space.

Pannach, F., Sporleder, C., May, W., Krishnan, A., & Sewchurran, A. (2021). Of lions and Yakshis. *Semantic Web*, 12(2), 219-239.

Propp, V. (1968). *Morphology of the folktale*. University of Texas Press.

Pianzola, F. (2018). Looking at narrative as a complex system: The proteus principle. In *Narrating complexity* (pp. 101-122).

Pianzola, F., Acerbi, A., & Rebora, S. (2020). Cultural accumulation and improvement in online fan fiction. In *CEUR Workshop Proceedings* (Vol. 2723). CEUR-WS. org.

Ryan, M.-L. (2019). Space. In P. Hühn et al. (Eds.), *The living handbook of narratology*. Hamburg University.

Sanfilippo, E. M., & Ferrario, R. (2024). D3.1—Observations modeling: State of the art.

Schöch, C., Hinzmann, M., Röttgermann, J., Dietz, K., & Klee, A. (2022). Smart modelling for literary history. *International Journal of Humanities and Arts Computing*, 16(1), 78–93.

Zgoll, A., Cuperly, B., & Cöster-Gilbert, A. (2023). In search of Dumuzi: An introduction to holistic narratology. In *The shape of stories* (pp. 285-350). Brill.

Zgoll, C. (2020). Myths as polymorphous and polystratic Erzählstoffe. In *Mythische Sphärenwechsel: Methodisch neue Zugänge zu antiken Mythen in Orient und Okzident* (pp. 9-82).""" .

#################################################################
#    Annotation properties
#################################################################

###  http://purl.org/dc/elements/1.1/date
dc:date rdf:type owl:AnnotationProperty .


###  http://purl.org/dc/elements/1.1/description
dc:description rdf:type owl:AnnotationProperty .


###  http://purl.org/dc/elements/1.1/title
dc:title rdf:type owl:AnnotationProperty .


###  http://www.w3.org/2000/01/rdf-schema#comment
rdfs:comment rdfs:comment "A description of the subject resource." ;
             rdfs:isDefinedBy rdfs: ;
             rdfs:label "comment" .


###  http://www.w3.org/2000/01/rdf-schema#isDefinedBy
rdfs:isDefinedBy rdfs:comment "The defininition of the subject resource." ;
                 rdfs:isDefinedBy rdfs: ;
                 rdfs:label "isDefinedBy" .


###  http://www.w3.org/2000/01/rdf-schema#label
rdfs:label rdfs:comment "A human-readable name for the subject." ;
           rdfs:isDefinedBy rdfs: ;
           rdfs:label "label" .


###  http://www.w3.org/2000/01/rdf-schema#seeAlso
rdfs:seeAlso rdfs:comment "Further information about the subject resource." ;
             rdfs:isDefinedBy rdfs: ;
             rdfs:label "seeAlso" .


###  http://www.w3.org/2004/02/skos/core#example
skos:example rdf:type owl:AnnotationProperty .


###  http://www.w3.org/2004/02/skos/core#notation
skos:notation rdf:type owl:AnnotationProperty .


###  http://www.w3.org/2004/02/skos/core#prefLabel
skos:prefLabel rdf:type owl:AnnotationProperty .


#################################################################
#    Object Properties
#################################################################

###  http://iflastandards.info/ns/lrm/lrmoo/R3_is_realised_in
<http://iflastandards.info/ns/lrm/lrmoo/R3_is_realised_in> rdf:type owl:ObjectProperty ;
                                                           rdfs:subPropertyOf <http://www.cidoc-crm.org/cidoc-crm/P130_shows_features_of> ;
                                                           owl:inverseOf <http://iflastandards.info/ns/lrm/lrmoo/R3i_realises> ;
                                                           rdfs:domain <http://iflastandards.info/ns/lrm/lrmoo/F1_Work> ;
                                                           rdfs:range <http://iflastandards.info/ns/lrm/lrmoo/F2_Expression> ;
                                                           rdfs:comment """Quantification: one to many, necessary, dependent (1,n:1,1)

Scope note:
This property associates an instance of F2 Expression with an instance of F1 Work.
This property expresses the association that exists between an expression and the work that this expression conveys. Our factual knowledge of how a given work is historically realised into expressions is often limited. Therefore, this property makes it possible to express the association between an instance of F2 Expression and the instance of F1 Work it conveys without identifying the particular instances of F2 Expression that were part of a chain of derivation from the source."""@en ,
                                                                        "In GOLEM, a narrative or idea (work) is realized in a specific expression, such as a text, movie, performance, or other medium." ;
                                                           rdfs:label "R3 is realised in"@en ;
                                                           skos:example """The work Harry Potter and the Deathly Hallows (F1) is realised in the text of Harry Potter and the Deathly Hallows 
(Rowling, 2007) (F2).""" .


###  http://iflastandards.info/ns/lrm/lrmoo/R3i_realises
<http://iflastandards.info/ns/lrm/lrmoo/R3i_realises> rdf:type owl:ObjectProperty ;
                                                      rdfs:subPropertyOf <http://www.cidoc-crm.org/cidoc-crm/P130i_features_are_also_found_on> ;
                                                      rdfs:domain <http://iflastandards.info/ns/lrm/lrmoo/F2_Expression> ;
                                                      rdfs:range <http://iflastandards.info/ns/lrm/lrmoo/F1_Work> ;
                                                      rdfs:comment """Quantification of the inverse property: one to many, necessary, dependent (1,n:1,1)

Scope note of the inverse property:
This property associates an instance of F2 Expression with an instance of F1 Work.
This property expresses the association that exists between an expression and the work that this expression conveys. Our factual knowledge of how a given work is historically realised into expressions is often limited. Therefore, this property makes it possible to express the association between an instance of F2 Expression and the instance of F1 Work it conveys without identifying the particular instances of F2 Expression that were part of a chain of derivation from the source.

Examples of the inverse property:
- Agatha Christie’s work entitled ‘Murder on the Orient Express’ (F1) is realised in the original text written by Agatha Christie for the novel (F2).
- Agatha Christie’s work entitled ‘Murder on the Orient Express’ (F1) is realised in the German translation created by Elisabeth van Bebber (F2).
- Agatha Christie’s work entitled ‘Murder on the Orient Express’ (F1) is realised in the narration of the English text by David Suchet (F2).
- Dante’s work entitled ‘Inferno’ (F1) is realised in the Italian text of Dante’s ‘Inferno’ as found in the authoritative critical edition ‘La Commedia secondo l’antica issolu’ a cura di Giorgio Petrocchi, Milano: Mondadori, 1966-67 (= ‘Le Opere di Dante Alighieri’, Edizione Nazionale a cura della Società Dantesca Italiana, VII, 1-4) (F2).
- Johann Sebastian Bach’s ‘Goldberg Variations’ (F1) is realised in the score of the ‘Goldberg Variations’ (as published by Balthasar Schmid in 1741) (F2).
- Auguste Rodin’s work ‘The Thinker’ (F1) is realised in the first plaster version of ‘The thinker’ (F2) that Auguste Rodin made around 1881.
- Auguste Rodin’s work ‘The Thinker’ (F1) is realised in the large-scale version of ‘The thinker’ (F2) created at the Fonderie Alexis Rudier in 1904.
"""@en ,
                                                                   "A narrative or idea (work) is realized in a specific expression, such as a text, movie, performance, or other medium." ;
                                                      rdfs:label "R3i realises"@en ;
                                                      skos:notation "R3i" .


###  http://iflastandards.info/ns/lrm/lrmoo/R5_has_component
<http://iflastandards.info/ns/lrm/lrmoo/R5_has_component> rdf:type owl:ObjectProperty ;
                                                          owl:inverseOf <http://iflastandards.info/ns/lrm/lrmoo/R5i_is_component_of> ;
                                                          rdfs:domain <http://iflastandards.info/ns/lrm/lrmoo/F2_Expression> ;
                                                          rdfs:range <http://iflastandards.info/ns/lrm/lrmoo/F2_Expression> ;
                                                          rdfs:comment "In GOLEM, it indicates that an expression (such as a text) contains a specific component, like a word, sentence, or paragraph." ,
                                                                       """Quantification: many to many (0,n:0,n)

Scope note:
This property associates an instance of an F2 Expression X with a structural component Y that conveys a part of the overall work realized by X, such as volumes, chapters, or sections. This property is transitive, asymmetric and irreflexive.
Any part of an expression that conveys complete propositions, such as a single phrase, can be documented using the more general property P148 has component (is component of).
Any part of an expression that does not completely follow meaningful boundaries, such as lines or pages of text or portions visible on images, can be documented using the property P106 is composed of (forms part of), and not with R5 has component (is component of). Fragments, in particular, can be documented with the more specific property R15 has fragment (is fragment of).
This property does not cover the relationship that exists between expressions that are realisations of different works, where one is re-used in a new, larger expression. Such a relationship is modelled by R75 incorporates (is incorporated in)  ([LRMoo version1.0, 2024](https://www.cidoc-crm.org/extensions/lrmoo/html/LRMoo_v1.0.html)).""" ;
                                                          rdfs:label "R5 has component"@en ;
                                                          skos:example "Text of Harry Potter and the Deathly Hallows (Rowling, 2007) (F2) has component a paragraph in Harry Potter and the Deathly Hallows (F2)." .


###  http://iflastandards.info/ns/lrm/lrmoo/R5i_is_component_of
<http://iflastandards.info/ns/lrm/lrmoo/R5i_is_component_of> rdf:type owl:ObjectProperty ;
                                                             rdfs:domain <http://iflastandards.info/ns/lrm/lrmoo/F2_Expression> ;
                                                             rdfs:range <http://iflastandards.info/ns/lrm/lrmoo/F2_Expression> ;
                                                             rdfs:comment "In GOLEM, it indicates that an expression (such as a text) contains a specific component, like a word, sentence, or paragraph." ,
                                                                          """Quantification: many to many (0,n:0,n)

Scope note:
This property associates an instance of an F2 Expression X with a structural component Y that conveys a part of the overall work realized by X, such as volumes, chapters, or sections. This property is transitive, asymmetric and irreflexive.
Any part of an expression that conveys complete propositions, such as a single phrase, can be documented using the more general property P148 has component (is component of).
Any part of an expression that does not completely follow meaningful boundaries, such as lines or pages of text or portions visible on images, can be documented using the property P106 is composed of (forms part of), and not with R5 has component (is component of). Fragments, in particular, can be documented with the more specific property R15 has fragment (is fragment of).
This property does not cover the relationship that exists between expressions that are realisations of different works, where one is re-used in a new, larger expression. Such a relationship is modelled by R75 incorporates (is incorporated in)  ([LRMoo version1.0, 2024](https://www.cidoc-crm.org/extensions/lrmoo/html/LRMoo_v1.0.html)).""" ;
                                                             rdfs:label "R5i is component of"@en .


###  http://www.cidoc-crm.org/cidoc-crm/P127_has_broader_term
<http://www.cidoc-crm.org/cidoc-crm/P127_has_broader_term> rdf:type owl:ObjectProperty ;
                                                           owl:inverseOf <http://www.cidoc-crm.org/cidoc-crm/P127i_has_narrower_term> ;
                                                           rdfs:domain <http://www.cidoc-crm.org/cidoc-crm/E55_Type> ;
                                                           rdfs:range <http://www.cidoc-crm.org/cidoc-crm/E55_Type> ;
                                                           rdfs:comment """This property associates an instance of E55 Type with another instance of E55 Type that has a broader meaning.
It allows instances of E55 Types to be organised into hierarchies. This is the sense of “broader term generic (BTG)” as defined in ISO 25964-2:2013 (International Organization for Standardization 2013).
This property is transitive. This property is asymmetric  ([CIDOC-CRM version 7.1.3, 2024](https://cidoc-crm.org/html/cidoc_crm_v7.1.3.html))."""@en ;
                                                           rdfs:label "P127 has broader term"@en ;
                                                           skos:example "\"Friendship\" (E55) has broader term \"topic\" (E55)." .


###  http://www.cidoc-crm.org/cidoc-crm/P127i_has_narrower_term
<http://www.cidoc-crm.org/cidoc-crm/P127i_has_narrower_term> rdf:type owl:ObjectProperty ;
                                                             rdfs:domain <http://www.cidoc-crm.org/cidoc-crm/E55_Type> ;
                                                             rdfs:range <http://www.cidoc-crm.org/cidoc-crm/E55_Type> ;
                                                             rdfs:comment """This property associates an instance of E55 Type with another instance of E55 Type that has a broader meaning.
It allows instances of E55 Types to be organised into hierarchies. This is the sense of “broader term generic (BTG)” as defined in ISO 25964-2:2013 (International Organization for Standardization 2013).
This property is transitive. This property is asymmetric  ([CIDOC-CRM version 7.1.3, 2024](https://cidoc-crm.org/html/cidoc_crm_v7.1.3.html)).""" ;
                                                             rdfs:label "P127i has narrower term"@en .


###  http://www.cidoc-crm.org/cidoc-crm/P130_shows_features_of
<http://www.cidoc-crm.org/cidoc-crm/P130_shows_features_of> rdf:type owl:ObjectProperty ;
                                                            owl:inverseOf <http://www.cidoc-crm.org/cidoc-crm/P130i_features_are_also_found_on> ;
                                                            rdfs:domain <http://www.cidoc-crm.org/cidoc-crm/E70_Thing> ;
                                                            rdfs:range <http://www.cidoc-crm.org/cidoc-crm/E70_Thing> ;
                                                            rdfs:comment """This property generalises the notions of “copy of” and “similar to” into a directed relationship, where the domain expresses the derivative or influenced item and the range the source or influencing item, if such a direction can be established. The property can also be used to express similarity in cases that can be stated between two objects only, without historical knowledge about its reasons. The property expresses a symmetric relationship in case no direction of influence can be established either from evidence on the item itself or from historical knowledge. This holds in particular for siblings of a derivation process from a common source or non-causal cultural parallels, such as some weaving patterns.
The P130.1 kind of similarity property of the P130 shows features of (features are also found on) property enables the relationship between the domain and the range to be further clarified, in the sense from domain to range, if applicable. For example, it may be expressed if both items are product “of the same mould”, or if two texts “contain identical paragraphs”.
If the reason for similarity is a sort of derivation process, i.e. that the creator has used or had in mind the form of a particular thing during the creation or production, this process should be explicitly modelled. In these cases, P130 shows features of can be regarded as a shortcut of such a process. However, the current model does not contain any path specific enough to infer this property. Specializations of the CIDOC CRM may however be more explicit, for instance describing the use of moulds etc.
This property is not transitive. This property is irreflexive ([CIDOC-CRM version 7.1.3, 2024](https://cidoc-crm.org/html/cidoc_crm_v7.1.3.html))."""@en ,
                                                                         "In the GOLEM ontology, it indicates that a Stoff variant exhibits features of the Stoff, such as a Character-Stoff or Narrative-Stoff." ;
                                                            rdfs:label "P130 shows features of"@en ;
                                                            skos:example "Harry Potter (character) who appears in Harry Potter and the Philosopher's Stone (movie, 2001) (G1)  shows features of Harry Potter Stoff (G0)." ,
                                                                         "The Battle of Hogwarts in Harry Potter and the Deathly Hallows (Rowling, 2007) (G7) shows features of Battle of Hogwarts Stoff (G14)." .


###  http://www.cidoc-crm.org/cidoc-crm/P130i_features_are_also_found_on
<http://www.cidoc-crm.org/cidoc-crm/P130i_features_are_also_found_on> rdf:type owl:ObjectProperty ;
                                                                      rdfs:domain <http://www.cidoc-crm.org/cidoc-crm/E70_Thing> ;
                                                                      rdfs:range <http://www.cidoc-crm.org/cidoc-crm/E70_Thing> ;
                                                                      rdfs:comment "In the GOLEM ontology, it indicates that a Stoff variant exhibits features of the Stoff, such as a Character-Stoff or Narrative-Stoff." ,
                                                                                   """This property generalises the notions of “copy of” and “similar to” into a directed relationship, where the domain expresses the derivative or influenced item and the range the source or influencing item, if such a direction can be established. The property can also be used to express similarity in cases that can be stated between two objects only, without historical knowledge about its reasons. The property expresses a symmetric relationship in case no direction of influence can be established either from evidence on the item itself or from historical knowledge. This holds in particular for siblings of a derivation process from a common source or non-causal cultural parallels, such as some weaving patterns.
The P130.1 kind of similarity property of the P130 shows features of (features are also found on) property enables the relationship between the domain and the range to be further clarified, in the sense from domain to range, if applicable. For example, it may be expressed if both items are product “of the same mould”, or if two texts “contain identical paragraphs”.
If the reason for similarity is a sort of derivation process, i.e. that the creator has used or had in mind the form of a particular thing during the creation or production, this process should be explicitly modelled. In these cases, P130 shows features of can be regarded as a shortcut of such a process. However, the current model does not contain any path specific enough to infer this property. Specializations of the CIDOC CRM may however be more explicit, for instance describing the use of moulds etc.
This property is not transitive. This property is irreflexive ([CIDOC-CRM version 7.1.3, 2024](https://cidoc-crm.org/html/cidoc_crm_v7.1.3.html)).""" ;
                                                                      rdfs:label "P130i features are also found on"@en .


###  http://www.cidoc-crm.org/cidoc-crm/P140_assigned_attribute_to
<http://www.cidoc-crm.org/cidoc-crm/P140_assigned_attribute_to> rdf:type owl:ObjectProperty ;
                                                                owl:inverseOf <http://www.cidoc-crm.org/cidoc-crm/P140i_was_attributed_by> ;
                                                                rdfs:domain <http://www.cidoc-crm.org/cidoc-crm/E13_Attribute_Assignment> ;
                                                                rdfs:range <http://www.cidoc-crm.org/cidoc-crm/E1_CRM_Entity> ;
                                                                rdfs:comment """This property associates an instance of E13 Attribute Assignment with the instance of E1 CRM Entity about which it made an attribution. The instance of E1 CRM Entity plays the role of the domain of the attribution.
The kind of attribution made should be documented using P177 assigned property of type (is type of property assigned)  ([CIDOC-CRM version 7.1.3, 2024](https://cidoc-crm.org/html/cidoc_crm_v7.1.3.html))."""@en ;
                                                                rdfs:label "P140 assigned attribute to"@en ;
                                                                skos:example "Relationship assignment for Ron and Hermione (E13) assigned attribute to romantic love between Ron and Hermione (G4)." ,
                                                                             """The topic assignment for Harry Potter and the Philosopher's Stone (E13) assigned attribute to the work 
Harry Potter and the Philosopher's Stone (Rowling, 1997) (F1).""" .


###  http://www.cidoc-crm.org/cidoc-crm/P140i_was_attributed_by
<http://www.cidoc-crm.org/cidoc-crm/P140i_was_attributed_by> rdf:type owl:ObjectProperty ;
                                                             rdfs:domain <http://www.cidoc-crm.org/cidoc-crm/E1_CRM_Entity> ;
                                                             rdfs:range <http://www.cidoc-crm.org/cidoc-crm/E13_Attribute_Assignment> ;
                                                             rdfs:comment """This property associates an instance of E13 Attribute Assignment with the instance of E1 CRM Entity about which it made an attribution. The instance of E1 CRM Entity plays the role of the domain of the attribution.
The kind of attribution made should be documented using P177 assigned property of type (is type of property assigned)  ([CIDOC-CRM version 7.1.3, 2024](https://cidoc-crm.org/html/cidoc_crm_v7.1.3.html)).""" ;
                                                             rdfs:label "P140i was attributed by"@en .


###  http://www.cidoc-crm.org/cidoc-crm/P141_assigned
<http://www.cidoc-crm.org/cidoc-crm/P141_assigned> rdf:type owl:ObjectProperty ;
                                                   owl:inverseOf <http://www.cidoc-crm.org/cidoc-crm/P141i_was_assigned_by> ;
                                                   rdfs:domain <http://www.cidoc-crm.org/cidoc-crm/E13_Attribute_Assignment> ;
                                                   rdfs:range <http://www.cidoc-crm.org/cidoc-crm/E1_CRM_Entity> ;
                                                   rdfs:comment "This property associates an instance of E13 Attribute Assignment with the instance of E1 CRM Entity used in the attribution. The instance of E1 CRM Entity here plays the role of the range of the attribution. The kind of attribution made should be documented using P177 assigned property of type (is type of property assigned)  ([CIDOC-CRM version 7.1.3, 2024](https://cidoc-crm.org/html/cidoc_crm_v7.1.3.html))."@en ;
                                                   rdfs:label "P141 assigned"@en ;
                                                   skos:example "Relationship assignment for Ron and Hermione (E13) assigned Ron (G1) [to romantic love between Ron and Hermione (G4)]." ,
                                                                """The topic assignment for Harry Potter and the Philosopher's Stone (E13) assigned “friendship” (E55) [to the work 
Harry Potter and the Philosopher's Stone (F1)].""" .


###  http://www.cidoc-crm.org/cidoc-crm/P141i_was_assigned_by
<http://www.cidoc-crm.org/cidoc-crm/P141i_was_assigned_by> rdf:type owl:ObjectProperty ;
                                                           rdfs:domain <http://www.cidoc-crm.org/cidoc-crm/E1_CRM_Entity> ;
                                                           rdfs:range <http://www.cidoc-crm.org/cidoc-crm/E13_Attribute_Assignment> ;
                                                           rdfs:comment "This property associates an instance of E13 Attribute Assignment with the instance of E1 CRM Entity used in the attribution. The instance of E1 CRM Entity here plays the role of the range of the attribution. The kind of attribution made should be documented using P177 assigned property of type (is type of property assigned)  ([CIDOC-CRM version 7.1.3, 2024](https://cidoc-crm.org/html/cidoc_crm_v7.1.3.html))." ;
                                                           rdfs:label "P141i was assigned by"@en .


###  http://www.cidoc-crm.org/cidoc-crm/P16_used_specific_object
<http://www.cidoc-crm.org/cidoc-crm/P16_used_specific_object> rdf:type owl:ObjectProperty ;
                                                              owl:inverseOf <http://www.cidoc-crm.org/cidoc-crm/P16i_was_used_for> ;
                                                              rdfs:domain <http://www.cidoc-crm.org/cidoc-crm/E7_Activity> ;
                                                              rdfs:range <http://www.cidoc-crm.org/cidoc-crm/E70_Thing> ;
                                                              rdfs:comment "In GOLEM, indicates that an object (G16) is used in a narrative event (G5), or a source is used in an observation or inference process (E13)." ,
                                                                           """This property describes the use of material or immaterial things in a way essential to the performance or the outcome of an instance of E7 Activity.

This property typically applies to tools, instruments, moulds, raw materials and items embedded in a product. It implies that the presence of the object in question was a necessary condition for the action. For example, the activity of writing this text required the use of a computer. An immaterial thing can be used if at least one of its carriers is present. For example, the software tools on a computer.

Another example is the use of a particular name by a particular group of people over some span to identify a thing, such as a settlement. In this case, the physical carriers of this name are at least the people understanding its use  ([CIDOC-CRM version 7.1.3, 2024](https://cidoc-crm.org/html/cidoc_crm_v7.1.3.html)).""" ;
                                                              rdfs:label "P16 used specific object"@en .


###  http://www.cidoc-crm.org/cidoc-crm/P16i_was_used_for
<http://www.cidoc-crm.org/cidoc-crm/P16i_was_used_for> rdf:type owl:ObjectProperty ;
                                                       rdfs:domain <http://www.cidoc-crm.org/cidoc-crm/E70_Thing> ;
                                                       rdfs:range <http://www.cidoc-crm.org/cidoc-crm/E7_Activity> ;
                                                       rdfs:comment "In GOLEM, indicates that an object (G16) is used in a narrative event (G5), or a source is used in an observation or inference process (E13)." ,
                                                                    """This property describes the use of material or immaterial things in a way essential to the performance or the outcome of an instance of E7 Activity.

This property typically applies to tools, instruments, moulds, raw materials and items embedded in a product. It implies that the presence of the object in question was a necessary condition for the action. For example, the activity of writing this text required the use of a computer. An immaterial thing can be used if at least one of its carriers is present. For example, the software tools on a computer.

Another example is the use of a particular name by a particular group of people over some span to identify a thing, such as a settlement. In this case, the physical carriers of this name are at least the people understanding its use  ([CIDOC-CRM version 7.1.3, 2024](https://cidoc-crm.org/html/cidoc_crm_v7.1.3.html)).""" ;
                                                       rdfs:label "P16i was used for"@en ;
                                                       skos:example "The Elder Wand (G16) was used for the Battle of Hogwarts in Harry Potter and the Deathly Hallows (Rowling, 2007) (G5)." ,
                                                                    "The text of Harry Potter and the Philosopher's Stone (Rowling, 1997) was used for the assignment of the topic “friendship” (E13)." .


###  http://www.cidoc-crm.org/cidoc-crm/P177_assigned_property_of_type
<http://www.cidoc-crm.org/cidoc-crm/P177_assigned_property_of_type> rdf:type owl:ObjectProperty ;
                                                                    rdfs:subPropertyOf <http://www.cidoc-crm.org/cidoc-crm/P2_has_type> ;
                                                                    owl:inverseOf <http://www.cidoc-crm.org/cidoc-crm/P177i_is_type_of_property_assigned> ;
                                                                    rdfs:domain <http://www.cidoc-crm.org/cidoc-crm/E13_Attribute_Assignment> ;
                                                                    rdfs:range <http://www.cidoc-crm.org/cidoc-crm/E55_Type> ;
                                                                    rdfs:comment """This property associates an instance of E13 Attribute Assignment with the type of property or relation that this assignment maintains to hold between the item to which it assigns an attribute and the attribute itself. Note that the properties defined by the CIDOC CRM also constitute instances of E55 Type themselves. The direction of the assigned property of type is understood to be from the attributed item (the range of property P140 assigned attribute to) to the attribute item (the range of the property P141 assigned). More than one property type may be assigned to hold between two items.
A comprehensive explanation about refining CIDOC CRM concepts by E55 Type is given in the section “About Types” in the section on “Specific Modelling Constructs” of this document ([CIDOC-CRM version 7.1.3, 2024](https://cidoc-crm.org/html/cidoc_crm_v7.1.3.html))."""@en ,
                                                                                 "Links an attribution or statement-making process to the type of the object, attribute, or value." ;
                                                                    rdfs:label "P177 assigned property of type"@en ;
                                                                    skos:example "The topic assignment for Harry Potter and the Philosopher's Stone (E13) assigned property of type “topic” (E55)." .


###  http://www.cidoc-crm.org/cidoc-crm/P177i_is_type_of_property_assigned
<http://www.cidoc-crm.org/cidoc-crm/P177i_is_type_of_property_assigned> rdf:type owl:ObjectProperty ;
                                                                        rdfs:subPropertyOf <http://www.cidoc-crm.org/cidoc-crm/P2i_is_type_of> ;
                                                                        rdfs:domain <http://www.cidoc-crm.org/cidoc-crm/E55_Type> ;
                                                                        rdfs:range <http://www.cidoc-crm.org/cidoc-crm/E13_Attribute_Assignment> ;
                                                                        rdfs:comment """This property associates an instance of E13 Attribute Assignment with the type of property or relation that this assignment maintains to hold between the item to which it assigns an attribute and the attribute itself. Note that the properties defined by the CIDOC CRM also constitute instances of E55 Type themselves. The direction of the assigned property of type is understood to be from the attributed item (the range of property P140 assigned attribute to) to the attribute item (the range of the property P141 assigned). More than one property type may be assigned to hold between two items.
A comprehensive explanation about refining CIDOC CRM concepts by E55 Type is given in the section “About Types” in the section on “Specific Modelling Constructs” of this document ([CIDOC-CRM version 7.1.3, 2024](https://cidoc-crm.org/html/cidoc_crm_v7.1.3.html)).""" ;
                                                                        rdfs:label "P177i is type of property assigned"@en .


###  http://www.cidoc-crm.org/cidoc-crm/P2_has_type
<http://www.cidoc-crm.org/cidoc-crm/P2_has_type> rdf:type owl:ObjectProperty ;
                                                 owl:inverseOf <http://www.cidoc-crm.org/cidoc-crm/P2i_is_type_of> ;
                                                 rdfs:domain <http://www.cidoc-crm.org/cidoc-crm/E1_CRM_Entity> ;
                                                 rdfs:range <http://www.cidoc-crm.org/cidoc-crm/E55_Type> ;
                                                 rdfs:comment """This property allows sub-typing of CIDOC CRM entities –a form of specialisation – through the use of a terminological hierarchy, or thesaurus.
The CIDOC CRM is intended to focus on the high-level entities and relationships needed to describe data structures. Consequently, it does not specialise entities any further than is required for this immediate purpose. However, entities in the isA hierarchy of the CIDOC CRM may by specialised into any number of sub-entities, which can be defined in the E55 Type hierarchy. E41 Appellation, for example, may be specialised into “e-mail address”, “telephone number”, “post office box”, “URL”, etc., none of which figures explicitly in the CIDOC CRM class hierarchy. A comprehensive explanation about refining CIDOC CRM concepts by E55 Type is given in the section “About Types” in the section on “Specific Modelling Constructs” of this document.
This property is a shortcut for the path from E1 CRM Entity through P41i was classified by, E17 Type Assignment, P42 assigned to E55 Type ([CIDOC-CRM version 7.1.3, 2024](https://cidoc-crm.org/html/cidoc_crm_v7.1.3.html))."""@en ;
                                                 rdfs:label "P2 has type"@en ;
                                                 skos:example "Narrative function “Victory” (G10) has type “Proppian function” (E55)" .


###  http://www.cidoc-crm.org/cidoc-crm/P2i_is_type_of
<http://www.cidoc-crm.org/cidoc-crm/P2i_is_type_of> rdf:type owl:ObjectProperty ;
                                                    rdfs:domain <http://www.cidoc-crm.org/cidoc-crm/E55_Type> ;
                                                    rdfs:range <http://www.cidoc-crm.org/cidoc-crm/E1_CRM_Entity> ;
                                                    rdfs:comment """This property allows sub-typing of CIDOC CRM entities –a form of specialisation – through the use of a terminological hierarchy, or thesaurus.
The CIDOC CRM is intended to focus on the high-level entities and relationships needed to describe data structures. Consequently, it does not specialise entities any further than is required for this immediate purpose. However, entities in the isA hierarchy of the CIDOC CRM may by specialised into any number of sub-entities, which can be defined in the E55 Type hierarchy. E41 Appellation, for example, may be specialised into “e-mail address”, “telephone number”, “post office box”, “URL”, etc., none of which figures explicitly in the CIDOC CRM class hierarchy. A comprehensive explanation about refining CIDOC CRM concepts by E55 Type is given in the section “About Types” in the section on “Specific Modelling Constructs” of this document.
This property is a shortcut for the path from E1 CRM Entity through P41i was classified by, E17 Type Assignment, P42 assigned to E55 Type ([CIDOC-CRM version 7.1.3, 2024](https://cidoc-crm.org/html/cidoc_crm_v7.1.3.html)).""" ;
                                                    rdfs:label "P2i is type of"@en .


###  http://www.cidoc-crm.org/cidoc-crm/P43_has_dimension
<http://www.cidoc-crm.org/cidoc-crm/P43_has_dimension> rdf:type owl:ObjectProperty ;
                                                       owl:inverseOf <http://www.cidoc-crm.org/cidoc-crm/P43i_is_dimension_of> ;
                                                       rdfs:domain <http://www.cidoc-crm.org/cidoc-crm/E70_Thing> ;
                                                       rdfs:range <http://www.cidoc-crm.org/cidoc-crm/E54_Dimension> ;
                                                       rdfs:comment """This property records an instance of E54 Dimension of some instance of E70 Thing.
In the case that the recorded property is a result of a measurement of an instance of E18 Physical Thing, this property is a shortcut of the more fully developed path from E18 Physical Thing through P39i was measured by, E16 Measurement, P40 observed dimension to E54 Dimension.
It offers no information about how and when an E54 Dimension was established, nor by whom. Knowledge about an instance of E54 Dimension need not be the result of a measurement; it may be the result of evaluating data or other information, which should be documented as an instance of E13 Attribute Assignment.
An instance of E54 Dimension is specific to an instance of E70 Thing  ([CIDOC-CRM version 7.1.3, 2024](https://cidoc-crm.org/html/cidoc_crm_v7.1.3.html))."""@en ;
                                                       rdfs:label "P43 has dimension"@en .


###  http://www.cidoc-crm.org/cidoc-crm/P43i_is_dimension_of
<http://www.cidoc-crm.org/cidoc-crm/P43i_is_dimension_of> rdf:type owl:ObjectProperty ;
                                                          rdfs:domain <http://www.cidoc-crm.org/cidoc-crm/E54_Dimension> ;
                                                          rdfs:range <http://www.cidoc-crm.org/cidoc-crm/E70_Thing> ;
                                                          rdfs:comment """This property records an instance of E54 Dimension of some instance of E70 Thing.
In the case that the recorded property is a result of a measurement of an instance of E18 Physical Thing, this property is a shortcut of the more fully developed path from E18 Physical Thing through P39i was measured by, E16 Measurement, P40 observed dimension to E54 Dimension.
It offers no information about how and when an E54 Dimension was established, nor by whom. Knowledge about an instance of E54 Dimension need not be the result of a measurement; it may be the result of evaluating data or other information, which should be documented as an instance of E13 Attribute Assignment.
An instance of E54 Dimension is specific to an instance of E70 Thing  ([CIDOC-CRM version 7.1.3, 2024](https://cidoc-crm.org/html/cidoc_crm_v7.1.3.html)).""" ;
                                                          rdfs:label "P43i is dimension of"@en .


###  http://www.cidoc-crm.org/cidoc-crm/P67_refers_to
<http://www.cidoc-crm.org/cidoc-crm/P67_refers_to> rdf:type owl:ObjectProperty ;
                                                   rdfs:subPropertyOf owl:topObjectProperty ;
                                                   rdfs:domain <http://www.cidoc-crm.org/cidoc-crm/E89_Propositional_Object> ;
                                                   rdfs:range <http://www.cidoc-crm.org/cidoc-crm/E1_CRM_Entity> ;
                                                   rdfs:comment "In GOLEM, indicates that a narrative unit (G9) refers to a specific narrative event (G5)." ,
                                                                "This property documents that an instance of E89 Propositional Object makes a statement about an instance of E1 CRM Entity. P67 refers to (is referred to by) has the P67.1 has type link to an instance of E55 Type. This is intended to allow a more detailed description of the type of reference. This differs from P129 is about (is subject of), which describes the primary subject or subjects of the instance of E89 Propositional Object  ([CIDOC-CRM version 7.1.3, 2024](https://cidoc-crm.org/html/cidoc_crm_v7.1.3.html))." ;
                                                   rdfs:label "P67 refers to" ;
                                                   skos:example """The hyleme “Voldemort casts the ‘Avada Kedavra’ curse” (G9) refers to the event “Harry heard the high voice shriek 
[...]: ‘Avada Kedavra!’” (G5).""" .


###  http://www.cidoc-crm.org/cidoc-crm/P67i_is_referred_to_by
<http://www.cidoc-crm.org/cidoc-crm/P67i_is_referred_to_by> rdf:type owl:ObjectProperty ;
                                                            rdfs:subPropertyOf owl:topObjectProperty ;
                                                            rdfs:domain <http://www.cidoc-crm.org/cidoc-crm/E1_CRM_Entity> ;
                                                            rdfs:range <http://www.cidoc-crm.org/cidoc-crm/E89_Propositional_Object> ;
                                                            rdfs:comment "In GOLEM, indicates that a narrative unit (G9) refers to a specific narrative event (G5)." ,
                                                                         "This property documents that an instance of E89 Propositional Object makes a statement about an instance of E1 CRM Entity. P67 refers to (is referred to by) has the P67.1 has type link to an instance of E55 Type. This is intended to allow a more detailed description of the type of reference. This differs from P129 is about (is subject of), which describes the primary subject or subjects of the instance of E89 Propositional Object  ([CIDOC-CRM version 7.1.3, 2024](https://cidoc-crm.org/html/cidoc_crm_v7.1.3.html))." ;
                                                            rdfs:label "P67i is referred to by" .


###  http://www.cidoc-crm.org/cidoc-crm/P91_has_unit
<http://www.cidoc-crm.org/cidoc-crm/P91_has_unit> rdf:type owl:ObjectProperty ;
                                                  owl:inverseOf <http://www.cidoc-crm.org/cidoc-crm/P91i_is_unit_of> ;
                                                  rdfs:domain <http://www.cidoc-crm.org/cidoc-crm/E54_Dimension> ;
                                                  rdfs:range <http://www.cidoc-crm.org/cidoc-crm/E58_Measurement_Unit> ;
                                                  rdfs:comment "This property shows the type of unit an instance of E54 Dimension was expressed in." ;
                                                  rdfs:label "P91 has unit" ;
                                                  skos:example """Kudos (E54) has unit kudos (E58).
(Smile as Bright as the Sun as You Fade into Darkness from AO3)""" ,
                                                               "Word count (E54) has unit word count (E58)." .


###  http://www.cidoc-crm.org/cidoc-crm/P91i_is_unit_of
<http://www.cidoc-crm.org/cidoc-crm/P91i_is_unit_of> rdf:type owl:ObjectProperty ;
                                                     rdfs:domain <http://www.cidoc-crm.org/cidoc-crm/E58_Measurement_Unit> ;
                                                     rdfs:range <http://www.cidoc-crm.org/cidoc-crm/E54_Dimension> ;
                                                     rdfs:comment "This property shows the type of unit an instance of E54 Dimension was expressed in." ;
                                                     rdfs:label "P91i is unit of" .


###  http://www.loa-cnr.it/ontologies/CommonSenseMapping.owl#duration
<http://www.loa-cnr.it/ontologies/CommonSenseMapping.owl#duration> rdf:type owl:ObjectProperty ;
                                                                   rdfs:subPropertyOf <http://www.ontologydesignpatterns.org/ont/dlp/TemporalRelations.owl#temporal-location> ;
                                                                   owl:inverseOf <http://www.loa-cnr.it/ontologies/CommonSenseMapping.owl#duration-of> ;
                                                                   rdfs:domain <http://www.ontologydesignpatterns.org/ont/dlp/DOLCE-Lite.owl#perdurant> ;
                                                                   rdfs:range <http://www.ontologydesignpatterns.org/ont/dlp/DOLCE-Lite.owl#time-interval> ;
                                                                   rdfs:comment "In GOLEM, indicates that a narrative event (G5) has a specific duration." ,
                                                                                "The time interval of duration of a perdurant ([DOLCE-Lite-Plus, 2005](https://www.w3.org/2001/sw/BestPractices/WNET/DLP3941_daml.html))." ;
                                                                   rdfs:label "duration" ;
                                                                   skos:example "The Battle of Hogwarts (G5) has *duration* several hours (time-interval)." .


###  http://www.loa-cnr.it/ontologies/CommonSenseMapping.owl#duration-of
<http://www.loa-cnr.it/ontologies/CommonSenseMapping.owl#duration-of> rdf:type owl:ObjectProperty ;
                                                                      rdfs:subPropertyOf <http://www.ontologydesignpatterns.org/ont/dlp/TemporalRelations.owl#temporal-location-of> ;
                                                                      rdfs:domain <http://www.ontologydesignpatterns.org/ont/dlp/DOLCE-Lite.owl#time-interval> ;
                                                                      rdfs:range <http://www.ontologydesignpatterns.org/ont/dlp/DOLCE-Lite.owl#perdurant> ;
                                                                      rdfs:comment "In GOLEM, indicates that a narrative event (G5) has a specific duration." ,
                                                                                   "The time interval of duration of a perdurant ([DOLCE-Lite-Plus, 2005](https://www.w3.org/2001/sw/BestPractices/WNET/DLP3941_daml.html))." ;
                                                                      rdfs:label "duration of" .


###  http://www.ontologydesignpatterns.org/ont/dlp/DOLCE-Lite.owl#generic-dependent
<http://www.ontologydesignpatterns.org/ont/dlp/DOLCE-Lite.owl#generic-dependent> rdf:type owl:ObjectProperty ;
                                                                                 owl:inverseOf <http://www.ontologydesignpatterns.org/ont/dlp/DOLCE-Lite.owl#generically-dependent-on> ;
                                                                                 rdfs:domain <http://www.ontologydesignpatterns.org/ont/dlp/DOLCE-Lite.owl#particular> ;
                                                                                 rdfs:range <http://www.ontologydesignpatterns.org/ont/dlp/DOLCE-Lite.owl#particular> ;
                                                                                 rdfs:comment "In GOLEM, indicates that one entity is dependent on another, such as a relationship depending on an event or a narrative location (G13) depending on a physical location."@en ,
                                                                                              "The dependence on an individual of a given type at some time. This is traditionally a relation between particulars and universals, but this one states that x generically depends on y if a z different from y, but with the same properties, can be equivalently its depend-on. This is a temporally-indexed relation (embedded in this syntax) ([DOLCE-Lite-Plus, 2005](https://www.w3.org/2001/sw/BestPractices/WNET/DLP3941_daml.html))."@en ;
                                                                                 rdfs:label "generic dependent"@en .


###  http://www.ontologydesignpatterns.org/ont/dlp/DOLCE-Lite.owl#generic-location
<http://www.ontologydesignpatterns.org/ont/dlp/DOLCE-Lite.owl#generic-location> rdf:type owl:ObjectProperty ;
                                                                                owl:inverseOf <http://www.ontologydesignpatterns.org/ont/dlp/DOLCE-Lite.owl#generic-location-of> ;
                                                                                rdfs:domain <http://www.ontologydesignpatterns.org/ont/dlp/DOLCE-Lite.owl#particular> ;
                                                                                rdfs:range <http://www.ontologydesignpatterns.org/ont/dlp/DOLCE-Lite.owl#particular> ;
                                                                                rdfs:comment "In GOLEM, specifies the location (G13) of an enduring entity, such as a character (G1) or object (G16), within the narrative."@en ,
                                                                                             "The most generic location relation, probably equivalent to more than one image schema in a cognitive system (e.g. containment for exact location, proximity for approximate location). This is meant to reason on generalized, common sense as well as formal locations, including naive localization, between any kinds of entities. Generic location is branched into 'exact' location, ranging on regions, and 'approximate' (naive) location, ranging on non-regions  ([DOLCE-Lite-Plus, 2005](https://www.w3.org/2001/sw/BestPractices/WNET/DLP3941_daml.html))."@en ;
                                                                                rdfs:label "generic location"@en .


###  http://www.ontologydesignpatterns.org/ont/dlp/DOLCE-Lite.owl#generic-location-of
<http://www.ontologydesignpatterns.org/ont/dlp/DOLCE-Lite.owl#generic-location-of> rdf:type owl:ObjectProperty ;
                                                                                   rdfs:domain <http://www.ontologydesignpatterns.org/ont/dlp/DOLCE-Lite.owl#particular> ;
                                                                                   rdfs:range <http://www.ontologydesignpatterns.org/ont/dlp/DOLCE-Lite.owl#particular> ;
                                                                                   rdfs:comment "In GOLEM, specifies the location (G13) of an enduring entity, such as a character (G1) or object (G16), within the narrative."@en ,
                                                                                                "The most generic location relation, probably equivalent to more than one image schema in a cognitive system (e.g. containment for exact location, proximity for approximate location). This is meant to reason on generalized, common sense as well as formal locations, including naive localization, between any kinds of entities. Generic location is branched into 'exact' location, ranging on regions, and 'approximate' (naive) location, ranging on non-regions  ([DOLCE-Lite-Plus, 2005](https://www.w3.org/2001/sw/BestPractices/WNET/DLP3941_daml.html))."@en ;
                                                                                   rdfs:label "generic location of"@en ;
                                                                                   skos:example "Quidditch World Cup Campsite (G13) is generic location of Harry Potter (G1)." ,
                                                                                                "Quidditch World Cup Campsite (G13) is generic location of Quidditch banners and flags (G16)." .


###  http://www.ontologydesignpatterns.org/ont/dlp/DOLCE-Lite.owl#generically-dependent-on
<http://www.ontologydesignpatterns.org/ont/dlp/DOLCE-Lite.owl#generically-dependent-on> rdf:type owl:ObjectProperty ;
                                                                                        rdfs:domain <http://www.ontologydesignpatterns.org/ont/dlp/DOLCE-Lite.owl#particular> ;
                                                                                        rdfs:range <http://www.ontologydesignpatterns.org/ont/dlp/DOLCE-Lite.owl#particular> ;
                                                                                        rdfs:comment "In GOLEM, indicates that one entity is dependent on another, such as a relationship depending on an event or a narrative location (G13) depending on a physical location."@en ,
                                                                                                     "The dependence on an individual of a given type at some time. This is traditionally a relation between particulars and universals, but this one states that x generically depends on y if a z different from y, but with the same properties, can be equivalently its depend-on. This is a temporally-indexed relation (embedded in this syntax)  ([DOLCE-Lite-Plus, 2005](https://www.w3.org/2001/sw/BestPractices/WNET/DLP3941_daml.html))."@en ;
                                                                                        rdfs:label "generically dependent on"@en ;
                                                                                        skos:example "England in the Harry Potter series (G13) generically dependent on England in the real world (geographical-place)." ,
                                                                                                     "The romantic love between Ron and Hermione (G4) generically dependent on their kiss in the chamber of secrets (G5)." .


###  http://www.ontologydesignpatterns.org/ont/dlp/DOLCE-Lite.owl#participant
<http://www.ontologydesignpatterns.org/ont/dlp/DOLCE-Lite.owl#participant> rdf:type owl:ObjectProperty ;
                                                                           owl:inverseOf <http://www.ontologydesignpatterns.org/ont/dlp/DOLCE-Lite.owl#participant-in> ;
                                                                           rdfs:domain <http://www.ontologydesignpatterns.org/ont/dlp/DOLCE-Lite.owl#perdurant> ;
                                                                           rdfs:range <http://www.ontologydesignpatterns.org/ont/dlp/DOLCE-Lite.owl#endurant> ;
                                                                           rdfs:comment "In GOLEM, indicates that an endurant, such as a character (G1) or object (G16), participates in a specific narrative event (G5)."@en ,
                                                                                        "The immediate relation holding between endurants and perdurants (e.g. in 'the car is running'). Participation can be constant (in all parts of the perdurant, e.g. in 'the car is running'), or temporary (in only some parts, e.g. in 'I'm electing the president'). A 'functional' participant is specialized for those forms of participation that depend on the nature of participants, processes, or on the intentionality of agentive participants. Traditional 'thematic role' should be mapped to functional participation. For relations holding between participants in a same perdurant, see the co-participates relation  ([DOLCE-Lite-Plus, 2005](https://www.w3.org/2001/sw/BestPractices/WNET/DLP3941_daml.html))."@en ;
                                                                           rdfs:label "participant"@en .


###  http://www.ontologydesignpatterns.org/ont/dlp/DOLCE-Lite.owl#participant-in
<http://www.ontologydesignpatterns.org/ont/dlp/DOLCE-Lite.owl#participant-in> rdf:type owl:ObjectProperty ;
                                                                              rdfs:domain <http://www.ontologydesignpatterns.org/ont/dlp/DOLCE-Lite.owl#endurant> ;
                                                                              rdfs:range <http://www.ontologydesignpatterns.org/ont/dlp/DOLCE-Lite.owl#perdurant> ;
                                                                              rdfs:comment "In GOLEM, indicates that an endurant, such as a character (G1) or object (G16), participates in a specific narrative event (G5)."@en ,
                                                                                           "The immediate relation holding between endurants and perdurants (e.g. in 'the car is running'). Participation can be constant (in all parts of the perdurant, e.g. in 'the car is running'), or temporary (in only some parts, e.g. in 'I'm electing the president'). A 'functional' participant is specialized for those forms of participation that depend on the nature of participants, processes, or on the intentionality of agentive participants. Traditional 'thematic role' should be mapped to functional participation. For relations holding between participants in a same perdurant, see the co-participates relation  ([DOLCE-Lite-Plus, 2005](https://www.w3.org/2001/sw/BestPractices/WNET/DLP3941_daml.html))."@en ;
                                                                              rdfs:label "participant in"@en ;
                                                                              skos:example "Harry Potter (G1) participant in the Battle of Hogwarts (G5)." ,
                                                                                           "The egg (G16) participant in the event in which Cedric gives Harry a hint (G5) (chapter 24 of Harry Potter and the Goblet of Fire)." .


###  http://www.ontologydesignpatterns.org/ont/dlp/DOLCE-Lite.owl#proper-part
<http://www.ontologydesignpatterns.org/ont/dlp/DOLCE-Lite.owl#proper-part> rdf:type owl:ObjectProperty ;
                                                                           owl:inverseOf <http://www.ontologydesignpatterns.org/ont/dlp/DOLCE-Lite.owl#proper-part-of> ;
                                                                           rdfs:domain <http://www.ontologydesignpatterns.org/ont/dlp/DOLCE-Lite.owl#particular> ;
                                                                           rdfs:range <http://www.ontologydesignpatterns.org/ont/dlp/DOLCE-Lite.owl#particular> ;
                                                                           rdfs:comment "In GOLEM, indicates that an entity  is part of a larger entity. For example, a child location (G13) is part of a larger parent location (G13)." ,
                                                                                        "The proper part relation: irreflexive, antisymmetric, and transitive ([DOLCE-Lite-Plus, 2005](https://www.w3.org/2001/sw/BestPractices/WNET/DLP3941_daml.html))." ;
                                                                           rdfs:label "proper part"@en ;
                                                                           skos:example """Harry Potter and the Deathly Hallows (Rowling, 2007) (F1) has proper part Hyleme “Harry’s triumph, as Voldemort dies 
from his rebounded curse” (G9).""" ,
                                                                                        "Hogwarts School of Witchcraft and Wizardry (G13) has proper part  Forbidden Forest (G13)." .


###  http://www.ontologydesignpatterns.org/ont/dlp/DOLCE-Lite.owl#proper-part-of
<http://www.ontologydesignpatterns.org/ont/dlp/DOLCE-Lite.owl#proper-part-of> rdf:type owl:ObjectProperty ;
                                                                              rdfs:domain <http://www.ontologydesignpatterns.org/ont/dlp/DOLCE-Lite.owl#particular> ;
                                                                              rdfs:range <http://www.ontologydesignpatterns.org/ont/dlp/DOLCE-Lite.owl#particular> ;
                                                                              rdfs:comment "In GOLEM, indicates that an entity  is part of a larger entity. For example, a child location (G13) is part of a larger parent location (G13)." ,
                                                                                           "The proper part relation: irreflexive, antisymmetric, and transitive ([DOLCE-Lite-Plus, 2005](https://www.w3.org/2001/sw/BestPractices/WNET/DLP3941_daml.html))." ;
                                                                              rdfs:label "proper part of"@en .


###  http://www.ontologydesignpatterns.org/ont/dlp/ExtendedDnS.owl#d-used-by
<http://www.ontologydesignpatterns.org/ont/dlp/ExtendedDnS.owl#d-used-by> rdf:type owl:ObjectProperty ;
                                                                          owl:inverseOf <http://www.ontologydesignpatterns.org/ont/dlp/ExtendedDnS.owl#d-uses> ;
                                                                          rdfs:domain <http://www.ontologydesignpatterns.org/ont/dlp/ExtendedDnS.owl#concept> ,
                                                                                      <http://www.ontologydesignpatterns.org/ont/dlp/ExtendedDnS.owl#role> ;
                                                                          rdfs:range <http://www.ontologydesignpatterns.org/ont/dlp/ExtendedDnS.owl#description> ;
                                                                          rdfs:comment "This property links a (dlp:)description, such as a work (F1) or relationship (G4), to a (dlp:)role, like a narrative function (G10) or a relationship role (G6). It also  links a work (F1) to a (dlp:)course, like fabula (G7) or syuzhet (G8)."@en ,
                                                                                       """Descriptions can d-use (descriptively use) concepts or figures, provided that used ones are defined by some description
([DOLCE-Lite-Plus, 2005](https://www.w3.org/2001/sw/BestPractices/WNET/DLP3941_daml.html)).""" ;
                                                                          rdfs:label "d-used-by"@en .


###  http://www.ontologydesignpatterns.org/ont/dlp/ExtendedDnS.owl#d-uses
<http://www.ontologydesignpatterns.org/ont/dlp/ExtendedDnS.owl#d-uses> rdf:type owl:ObjectProperty ;
                                                                       rdfs:domain <http://www.ontologydesignpatterns.org/ont/dlp/ExtendedDnS.owl#description> ;
                                                                       rdfs:range <http://www.ontologydesignpatterns.org/ont/dlp/ExtendedDnS.owl#concept> ,
                                                                                  <http://www.ontologydesignpatterns.org/ont/dlp/ExtendedDnS.owl#role> ;
                                                                       rdfs:comment "This property links a (dlp:)description, such as a work (F1) or relationship (G4), to a (dlp:)role, like a narrative function (G10) or a relationship role (G6). It also  links a work (F1) to a (dlp:)course, like fabula (G7) or syuzhet (G8)."@en ,
                                                                                    """Descriptions can d-use (descriptively use) concepts or figures, provided that used ones are defined by some description
([DOLCE-Lite-Plus, 2005](https://www.w3.org/2001/sw/BestPractices/WNET/DLP3941_daml.html)).""" ;
                                                                       rdfs:label "d-uses"@en ;
                                                                       skos:example "Harry Potter and the Deathly Hallows (Rowling, 2007) (F1) d-uses the fabula of Harry Potter and the Deathly Hallows (G7)." ,
                                                                                    "Romantic love between Ron and Hermione (G4) d-uses the role \"lover\" (G6)." .


###  http://www.ontologydesignpatterns.org/ont/dlp/ExtendedDnS.owl#involved-in
<http://www.ontologydesignpatterns.org/ont/dlp/ExtendedDnS.owl#involved-in> rdf:type owl:ObjectProperty ;
                                                                            owl:inverseOf <http://www.ontologydesignpatterns.org/ont/dlp/ExtendedDnS.owl#involves> ;
                                                                            rdfs:domain <http://www.ontologydesignpatterns.org/ont/dlp/DOLCE-Lite.owl#endurant> ;
                                                                            rdfs:range <http://www.ontologydesignpatterns.org/ont/dlp/ExtendedDnS.owl#description> ;
                                                                            rdfs:comment "In GOLEM, indicates that a character is involved in a social relationship."@en ,
                                                                                         "The composition of d-uses and played-by relations: a description d-uses a role that is played by an endurant  ([DOLCE-Lite-Plus, 2005](https://www.w3.org/2001/sw/BestPractices/WNET/DLP3941_daml.html))."@en ;
                                                                            rdfs:label "involved in"@en ;
                                                                            skos:example "Ron (G1) involved in the romantic love between Ron and Hermione (G4)." .


###  http://www.ontologydesignpatterns.org/ont/dlp/ExtendedDnS.owl#involves
<http://www.ontologydesignpatterns.org/ont/dlp/ExtendedDnS.owl#involves> rdf:type owl:ObjectProperty ;
                                                                         rdfs:domain <http://www.ontologydesignpatterns.org/ont/dlp/ExtendedDnS.owl#description> ;
                                                                         rdfs:range <http://www.ontologydesignpatterns.org/ont/dlp/DOLCE-Lite.owl#endurant> ;
                                                                         rdfs:comment "In GOLEM, indicates that a character is involved in a social relationship."@en ,
                                                                                      "The composition of d-uses and played-by relations: a description d-uses a role that is played by an endurant  ([DOLCE-Lite-Plus, 2005](https://www.w3.org/2001/sw/BestPractices/WNET/DLP3941_daml.html))."@en ;
                                                                         rdfs:label "involves"@en .


###  http://www.ontologydesignpatterns.org/ont/dlp/ExtendedDnS.owl#modal-target
<http://www.ontologydesignpatterns.org/ont/dlp/ExtendedDnS.owl#modal-target> rdf:type owl:ObjectProperty ;
                                                                             owl:inverseOf <http://www.ontologydesignpatterns.org/ont/dlp/ExtendedDnS.owl#modal-target-of> ;
                                                                             rdfs:domain <http://www.ontologydesignpatterns.org/ont/dlp/ExtendedDnS.owl#role> ;
                                                                             rdfs:range <http://www.ontologydesignpatterns.org/ont/dlp/ExtendedDnS.owl#course> ;
                                                                             rdfs:comment "The relation between roles and courses. Modal target subrelations can be seen as 'reifications' of the operators of modal logics  ([DOLCE-Lite-Plus, 2005](https://www.w3.org/2001/sw/BestPractices/WNET/DLP3941_daml.html))."@en ,
                                                                                          "In GOLEM, relates a sequence of narrative events (dlp:perdurants), like fabula (G7) or syuzhet (G8), to its target narrative function (G10) or relationship role (G11). This property is useful both to link tropes to the whole course of action of a story and to retrieve all the narrative functions associated with the events of a story." ;
                                                                             rdfs:label "modal target"@en .


###  http://www.ontologydesignpatterns.org/ont/dlp/ExtendedDnS.owl#modal-target-of
<http://www.ontologydesignpatterns.org/ont/dlp/ExtendedDnS.owl#modal-target-of> rdf:type owl:ObjectProperty ;
                                                                                rdfs:domain <http://www.ontologydesignpatterns.org/ont/dlp/ExtendedDnS.owl#course> ;
                                                                                rdfs:range <http://www.ontologydesignpatterns.org/ont/dlp/ExtendedDnS.owl#role> ;
                                                                                rdfs:comment "The relation between roles and courses. Modal target subrelations can be seen as 'reifications' of the operators of modal logics  ([DOLCE-Lite-Plus, 2005](https://www.w3.org/2001/sw/BestPractices/WNET/DLP3941_daml.html))."@en ,
                                                                                             "In GOLEM, relates a sequence of narrative events (dlp:perdurants), like fabula (G7) or syuzhet (G8), to its target narrative function (G10) or relationship role (G11). This property is useful both to link tropes to the whole course of action of a story and to retrieve all the narrative functions associated with the events of a story." ;
                                                                                rdfs:label "modal target of"@en ;
                                                                                skos:example "Proppian function “Victory” (G10) is the modal target of the fabula  (G7) of Harry Potter and the Deathly Hallows (Rowling, 2007)." ,
                                                                                             "“Hero” (G11) is modal target of the syuzhet (G8) of Battle of Hogwarts in Harry Potter and the Deathly Hallows (Rowling, 2007)." .


###  http://www.ontologydesignpatterns.org/ont/dlp/ExtendedDnS.owl#played-by
<http://www.ontologydesignpatterns.org/ont/dlp/ExtendedDnS.owl#played-by> rdf:type owl:ObjectProperty ;
                                                                          owl:inverseOf <http://www.ontologydesignpatterns.org/ont/dlp/ExtendedDnS.owl#plays> ;
                                                                          rdfs:domain <http://www.ontologydesignpatterns.org/ont/dlp/ExtendedDnS.owl#role> ;
                                                                          rdfs:range <http://www.ontologydesignpatterns.org/ont/dlp/DOLCE-Lite.owl#endurant> ;
                                                                          rdfs:comment "In GOLEM, an endurant, such as a narrative unit or a character, plays a role in a (dlp:)description, such as a narrative function (G10) or relationship role (G11)." ,
                                                                                       "This is the immediate relation between roles and endurants. A role selects the position (function, use, relevance, ...) of an endurant within a context (s-description). Roles can be ordered, interdependent, at different layers. etc. ([DOLCE-Lite-Plus, 2005](https://www.w3.org/2001/sw/BestPractices/WNET/DLP3941_daml.html))." ;
                                                                          rdfs:label "played-by"@en .


###  http://www.ontologydesignpatterns.org/ont/dlp/ExtendedDnS.owl#plays
<http://www.ontologydesignpatterns.org/ont/dlp/ExtendedDnS.owl#plays> rdf:type owl:ObjectProperty ;
                                                                      rdfs:domain <http://www.ontologydesignpatterns.org/ont/dlp/DOLCE-Lite.owl#endurant> ;
                                                                      rdfs:range <http://www.ontologydesignpatterns.org/ont/dlp/ExtendedDnS.owl#role> ;
                                                                      rdfs:comment "In GOLEM, an endurant, such as a narrative unit or a character, plays a role in a (dlp:)description, such as a narrative function (G10) or relationship role (G11)." ,
                                                                                   "This is the immediate relation between roles and endurants. A role selects the position (function, use, relevance, ...) of an endurant within a context (s-description). Roles can be ordered, interdependent, at different layers. etc.  ([DOLCE-Lite-Plus, 2005](https://www.w3.org/2001/sw/BestPractices/WNET/DLP3941_daml.html))." ;
                                                                      rdfs:label "plays"@en ;
                                                                      skos:example "Ron (G1) plays relationship role \"lover\" (G4)." ,
                                                                                   "The hyper-hyleme \"Harry defeats Voldemort” (G9) plays proppian function \"Victory\" (G10)." .


###  http://www.ontologydesignpatterns.org/ont/dlp/ExtendedDnS.owl#predecessor
<http://www.ontologydesignpatterns.org/ont/dlp/ExtendedDnS.owl#predecessor> rdf:type owl:ObjectProperty ;
                                                                            owl:inverseOf <http://www.ontologydesignpatterns.org/ont/dlp/ExtendedDnS.owl#successor> ;
                                                                            rdf:type owl:TransitiveProperty ;
                                                                            rdfs:domain <http://www.ontologydesignpatterns.org/ont/dlp/DOLCE-Lite.owl#particular> ;
                                                                            rdfs:range <http://www.ontologydesignpatterns.org/ont/dlp/DOLCE-Lite.owl#particular> ;
                                                                            rdfs:comment "Specifies the order between two entities, where one is the successor or predecessor of the other." ,
                                                                                         "To be understood as 'entity x  has predecessor y'.This is the transitive version, but it results to be a complex property in OWL-DL, and transitivity should be overruled ([DOLCE-Lite-Plus, 2005](https://www.w3.org/2001/sw/BestPractices/WNET/DLP3941_daml.html))." ;
                                                                            rdfs:label "predecessor" ;
                                                                            skos:example "Harry's life at the Dursleys (G12) is predecessor of the Wizarding World (G12)." .


###  http://www.ontologydesignpatterns.org/ont/dlp/ExtendedDnS.owl#satisfied-by
<http://www.ontologydesignpatterns.org/ont/dlp/ExtendedDnS.owl#satisfied-by> rdf:type owl:ObjectProperty ;
                                                                             owl:inverseOf <http://www.ontologydesignpatterns.org/ont/dlp/ExtendedDnS.owl#satisfies> ;
                                                                             rdfs:domain <http://www.ontologydesignpatterns.org/ont/dlp/ExtendedDnS.owl#description> ;
                                                                             rdfs:range <http://www.ontologydesignpatterns.org/ont/dlp/ExtendedDnS.owl#situation> ;
                                                                             rdfs:comment "In GOLEM, this property links  a setting (G12) to  a work (F1)." ,
                                                                                          "See also comment on 'satisfies' for a different explanation. This is the primitive relation between descriptions and situations. It can be understood as a reification of the 'satisfiability' relation of formal semantics that holds between theories and models. A theory is reified as an description, thus acquiring a life-cycle: a theory can be changed, versioned, discussed, issued, etc. 'Theory' can be a 'potential' theory in the sense that most conceptualizations that could be formalized, could also be reified, e.g. plans, norms, stories, projects, diagnoses, methods, etc. No position is taken on the extensionality of descriptions. For example, if a theory is required to be reified in fine detail, if it changes an axiom, it could be considered no more the same theory. On the other hand, if theories are reified without such a strong assumption, some axioms can be changed just like non-essential parts of physical objects, with the theory preserving its identity. In case a theory is considered extensional, it might be considered a member of a class of 'theory changing history'. The 'refines' relation provides this possibility. A model is reified as a situation, thus a *class* of models that can satisfy a theory are reified as a situation type (class). Situations can depend on descriptions, but not vice-versa (constructivist stance). Components of descriptions 'select' entities of situations. There are at least three satisfaction subrelations, and a lot of conditions can be stated for allowing an automatic matching of satisfaction. See the FOL version of DLP for details ([DOLCE-Lite-Plus, 2005](https://www.w3.org/2001/sw/BestPractices/WNET/DLP3941_daml.html))." ;
                                                                             rdfs:label "satisfied by"@en .


###  http://www.ontologydesignpatterns.org/ont/dlp/ExtendedDnS.owl#satisfies
<http://www.ontologydesignpatterns.org/ont/dlp/ExtendedDnS.owl#satisfies> rdf:type owl:ObjectProperty ;
                                                                          rdfs:domain <http://www.ontologydesignpatterns.org/ont/dlp/ExtendedDnS.owl#situation> ;
                                                                          rdfs:range <http://www.ontologydesignpatterns.org/ont/dlp/ExtendedDnS.owl#description> ;
                                                                          rdfs:comment "In GOLEM, this property links  a setting (G12) to  a work (F1)." ,
                                                                                       "See also comment on 'satisfies' for a different explanation. This is the primitive relation between descriptions and situations. It can be understood as a reification of the 'satisfiability' relation of formal semantics that holds between theories and models. A theory is reified as an description, thus acquiring a life-cycle: a theory can be changed, versioned, discussed, issued, etc. 'Theory' can be a 'potential' theory in the sense that most conceptualizations that could be formalized, could also be reified, e.g. plans, norms, stories, projects, diagnoses, methods, etc. No position is taken on the extensionality of descriptions. For example, if a theory is required to be reified in fine detail, if it changes an axiom, it could be considered no more the same theory. On the other hand, if theories are reified without such a strong assumption, some axioms can be changed just like non-essential parts of physical objects, with the theory preserving its identity. In case a theory is considered extensional, it might be considered a member of a class of 'theory changing history'. The 'refines' relation provides this possibility. A model is reified as a situation, thus a *class* of models that can satisfy a theory are reified as a situation type (class). Situations can depend on descriptions, but not vice-versa (constructivist stance). Components of descriptions 'select' entities of situations. There are at least three satisfaction subrelations, and a lot of conditions can be stated for allowing an automatic matching of satisfaction. See the FOL version of DLP for details ([DOLCE-Lite-Plus, 2005](https://www.w3.org/2001/sw/BestPractices/WNET/DLP3941_daml.html))." ;
                                                                          rdfs:label "satisfies"@en ;
                                                                          skos:example """The setting of \"Wizarding community rivalries during the Triwizard Tournament\" (G12) satisfies the work Harry Potter 
and the Goblet of Fire (F1).""" .


###  http://www.ontologydesignpatterns.org/ont/dlp/ExtendedDnS.owl#sequenced-by
<http://www.ontologydesignpatterns.org/ont/dlp/ExtendedDnS.owl#sequenced-by> rdf:type owl:ObjectProperty ;
                                                                             owl:inverseOf <http://www.ontologydesignpatterns.org/ont/dlp/ExtendedDnS.owl#sequences> ;
                                                                             rdfs:domain <http://www.ontologydesignpatterns.org/ont/dlp/ExtendedDnS.owl#course> ;
                                                                             rdfs:range <http://www.ontologydesignpatterns.org/ont/dlp/DOLCE-Lite.owl#perdurant> ;
                                                                             rdfs:comment "In GOLEM, indicates that a fabula (G7) or syuzhet (G8) sequences narrative events in a specific order." ,
                                                                                          "This is the immediate relation between courses and perdurants. A course can be either atomic, being a simple 'perdurant role', or it can be complex, thus creating an abstract ordering over a temporal or causal sequence of processes or actions. The ontology of plans develops in detail intentional complex courses ([DOLCE-Lite-Plus, 2005](https://www.w3.org/2001/sw/BestPractices/WNET/DLP3941_daml.html))." ;
                                                                             rdfs:label "sequenced-by"@en .


###  http://www.ontologydesignpatterns.org/ont/dlp/ExtendedDnS.owl#sequences
<http://www.ontologydesignpatterns.org/ont/dlp/ExtendedDnS.owl#sequences> rdf:type owl:ObjectProperty ;
                                                                          rdfs:domain <http://www.ontologydesignpatterns.org/ont/dlp/DOLCE-Lite.owl#perdurant> ;
                                                                          rdfs:range <http://www.ontologydesignpatterns.org/ont/dlp/ExtendedDnS.owl#course> ;
                                                                          rdfs:comment "In GOLEM, indicates that a fabula (G7) or syuzhet (G8) sequences narrative events in a specific order." ,
                                                                                       "This is the immediate relation between courses and perdurants. A course can be either atomic, being a simple 'perdurant role', or it can be complex, thus creating an abstract ordering over a temporal or causal sequence of processes or actions. The ontology of plans develops in detail intentional complex courses ([DOLCE-Lite-Plus, 2005](https://www.w3.org/2001/sw/BestPractices/WNET/DLP3941_daml.html))." ;
                                                                          rdfs:label "sequences"@en ;
                                                                          skos:example "The fabula (G7) and syuzhet (G8) of Battle of Hogwarts in Harry Potter and the Deathly Hallows (J. K. Rowling, 2007) sequences a series of individual events" .


###  http://www.ontologydesignpatterns.org/ont/dlp/ExtendedDnS.owl#setting
<http://www.ontologydesignpatterns.org/ont/dlp/ExtendedDnS.owl#setting> rdf:type owl:ObjectProperty ;
                                                                        owl:inverseOf <http://www.ontologydesignpatterns.org/ont/dlp/ExtendedDnS.owl#setting-for> ;
                                                                        rdfs:domain <http://www.ontologydesignpatterns.org/ont/dlp/DOLCE-Lite.owl#particular> ;
                                                                        rdfs:range <http://www.ontologydesignpatterns.org/ont/dlp/ExtendedDnS.owl#situation> ;
                                                                        rdfs:comment "In GOLEM, links a narrative setting (G12) to various elements such as location (G13), time, character (G1), object (G16), or event (G5)." ,
                                                                                     "The relation between a situation and the entities that constitute it. (At least some of, or all) such entities must be classified by concepts defined by the description that the situation is supposed to satisfy ([DOLCE-Lite-Plus, 2005](https://www.w3.org/2001/sw/BestPractices/WNET/DLP3941_daml.html))." ;
                                                                        rdfs:label "setting"@en .


###  http://www.ontologydesignpatterns.org/ont/dlp/ExtendedDnS.owl#setting-for
<http://www.ontologydesignpatterns.org/ont/dlp/ExtendedDnS.owl#setting-for> rdf:type owl:ObjectProperty ;
                                                                            rdfs:domain <http://www.ontologydesignpatterns.org/ont/dlp/ExtendedDnS.owl#situation> ;
                                                                            rdfs:range <http://www.ontologydesignpatterns.org/ont/dlp/DOLCE-Lite.owl#particular> ;
                                                                            rdfs:comment "In GOLEM, links a narrative setting (G12) to various elements such as location (G13), time, character (G1), object (G16), or event (G5)." ,
                                                                                         "The relation between a situation and the entities that constitute it. (At least some of, or all) such entities must be classified by concepts defined by the description that the situation is supposed to satisfy ([DOLCE-Lite-Plus, 2005](https://www.w3.org/2001/sw/BestPractices/WNET/DLP3941_daml.html))." ;
                                                                            rdfs:label "setting for"@en ;
                                                                            skos:example "Wizarding community rivalries during the Triwizard Tournament (G12) is setting for Harry Potter (G1)." ,
                                                                                         "Wizarding community rivalries during the Triwizard Tournament (G12) is setting for Quidditch World Cup campsite (G13)." ,
                                                                                         "Wizarding community rivalries during the Triwizard Tournament (G12) is setting for Triwizard Tournament (G5)." .


###  http://www.ontologydesignpatterns.org/ont/dlp/ExtendedDnS.owl#successor
<http://www.ontologydesignpatterns.org/ont/dlp/ExtendedDnS.owl#successor> rdf:type owl:ObjectProperty ,
                                                                                   owl:TransitiveProperty ;
                                                                          rdfs:domain <http://www.ontologydesignpatterns.org/ont/dlp/DOLCE-Lite.owl#particular> ;
                                                                          rdfs:range <http://www.ontologydesignpatterns.org/ont/dlp/DOLCE-Lite.owl#particular> ;
                                                                          rdfs:comment "Specifies the order between two entities, where one is the successor or predecessor of the other." ,
                                                                                       "To be understood as 'entity x  has predecessor y'.This is the transitive version, but it results to be a complex property in OWL-DL, and transitivity should be overruled ([DOLCE-Lite-Plus, 2005](https://www.w3.org/2001/sw/BestPractices/WNET/DLP3941_daml.html))." ;
                                                                          rdfs:label "successor"@en .


###  http://www.ontologydesignpatterns.org/ont/dlp/ExtendedDnS.owl#used-by
<http://www.ontologydesignpatterns.org/ont/dlp/ExtendedDnS.owl#used-by> rdf:type owl:ObjectProperty ;
                                                                        owl:inverseOf <http://www.ontologydesignpatterns.org/ont/dlp/ExtendedDnS.owl#uses> ;
                                                                        rdfs:domain <http://www.ontologydesignpatterns.org/ont/dlp/DOLCE-Lite.owl#endurant> ;
                                                                        rdfs:range <http://www.ontologydesignpatterns.org/ont/dlp/DOLCE-Lite.owl#endurant> ;
                                                                        rdfs:comment "In GOLEM, describes a character's (G1) use of an object (G16) in a narrative event (G5) or narrative unit (G9)." ,
                                                                                     "The use relations between endurants: an endurant e1 uses e2 within a perdurant in which both are participating. A rule then states that if e1 uses e2, e2 is used *in* a perdurant ([DOLCE-Lite-Plus, 2005](https://www.w3.org/2001/sw/BestPractices/WNET/DLP3941_daml.html))." ;
                                                                        rdfs:label "used-by"@en .


###  http://www.ontologydesignpatterns.org/ont/dlp/ExtendedDnS.owl#uses
<http://www.ontologydesignpatterns.org/ont/dlp/ExtendedDnS.owl#uses> rdf:type owl:ObjectProperty ;
                                                                     rdfs:domain <http://www.ontologydesignpatterns.org/ont/dlp/DOLCE-Lite.owl#endurant> ;
                                                                     rdfs:range <http://www.ontologydesignpatterns.org/ont/dlp/DOLCE-Lite.owl#endurant> ;
                                                                     rdfs:comment "In GOLEM, describes a character's (G1) use of an object (G16) in a narrative event (G5) or narrative unit (G9)." ,
                                                                                  "The use relations between endurants: an endurant e1 uses e2 within a perdurant in which both are participating. A rule then states that if e1 uses e2, e2 is used *in* a perdurant ([DOLCE-Lite-Plus, 2005](https://www.w3.org/2001/sw/BestPractices/WNET/DLP3941_daml.html))." ;
                                                                     rdfs:label "uses"@en ;
                                                                     skos:example "Harry Potter (G1) uses the Elder Wand (G16) in the Battle of Hogwarts." .


###  http://www.ontologydesignpatterns.org/ont/dlp/FunctionalParticipation.owl#has-state
<http://www.ontologydesignpatterns.org/ont/dlp/FunctionalParticipation.owl#has-state> rdf:type owl:ObjectProperty ;
                                                                                      owl:inverseOf <http://www.ontologydesignpatterns.org/ont/dlp/FunctionalParticipation.owl#state-of> ;
                                                                                      rdfs:domain <http://www.ontologydesignpatterns.org/ont/dlp/DOLCE-Lite.owl#endurant> ;
                                                                                      rdfs:range <http://www.ontologydesignpatterns.org/ont/dlp/DOLCE-Lite.owl#state> ;
                                                                                      rdfs:comment "Participation in a state  ([DOLCE-Lite-Plus, 2005](https://www.w3.org/2001/sw/BestPractices/WNET/DLP3941_daml.html))."@en ,
                                                                                                   "In GOLEM, indicates the psychological state (G3) of a character (G1)." ;
                                                                                      rdfs:label "has-state"@en ;
                                                                                      skos:example "Ron in Harry Potter and the Goblet of Fire (G1) has state “jealousy” (G3) during the event Yule Ball (G5)." .


###  http://www.ontologydesignpatterns.org/ont/dlp/FunctionalParticipation.owl#state-of
<http://www.ontologydesignpatterns.org/ont/dlp/FunctionalParticipation.owl#state-of> rdf:type owl:ObjectProperty ;
                                                                                     rdfs:domain <http://www.ontologydesignpatterns.org/ont/dlp/DOLCE-Lite.owl#state> ;
                                                                                     rdfs:range <http://www.ontologydesignpatterns.org/ont/dlp/DOLCE-Lite.owl#endurant> ;
                                                                                     rdfs:comment "In GOLEM, indicates the psychological state (G3) of a character (G1)." ,
                                                                                                  "Participation in a state ([DOLCE-Lite-Plus, 2005](https://www.w3.org/2001/sw/BestPractices/WNET/DLP3941_daml.html))." ;
                                                                                     rdfs:label "state-of"@en .


###  http://www.ontologydesignpatterns.org/ont/dlp/SpatialRelations.owl#participant-place
<http://www.ontologydesignpatterns.org/ont/dlp/SpatialRelations.owl#participant-place> rdf:type owl:ObjectProperty ;
                                                                                       owl:inverseOf <http://www.ontologydesignpatterns.org/ont/dlp/SpatialRelations.owl#participant-place-of> ;
                                                                                       rdfs:domain <http://www.ontologydesignpatterns.org/ont/dlp/DOLCE-Lite.owl#perdurant> ;
                                                                                       rdfs:range <http://www.ontologydesignpatterns.org/ont/dlp/DOLCE-Lite.owl#endurant> ;
                                                                                       rdfs:comment "In GOLEM, indicates the location (G13) where a narrative event (G5) took place."@en ,
                                                                                                    "The place of a perdurant as provided by a reference region at which the spatial quality of a certain endurant is q-located  ([DOLCE-Lite-Plus, 2005](https://www.w3.org/2001/sw/BestPractices/WNET/DLP3941_daml.html))."@en ;
                                                                                       rdfs:label "participant place"@en ;
                                                                                       skos:example "The Quidditch World Cup match (G5) has participant place Quidditch World Cup Campsite (G13)." .


###  http://www.ontologydesignpatterns.org/ont/dlp/SpatialRelations.owl#participant-place-of
<http://www.ontologydesignpatterns.org/ont/dlp/SpatialRelations.owl#participant-place-of> rdf:type owl:ObjectProperty ;
                                                                                          rdfs:domain <http://www.ontologydesignpatterns.org/ont/dlp/DOLCE-Lite.owl#endurant> ;
                                                                                          rdfs:range <http://www.ontologydesignpatterns.org/ont/dlp/DOLCE-Lite.owl#perdurant> ;
                                                                                          rdfs:comment "In GOLEM, indicates the location (G13) where a narrative event (G5) took place."@en ,
                                                                                                       "The place of a perdurant as provided by a reference region at which the spatial quality of a certain endurant is q-located  ([DOLCE-Lite-Plus, 2005](https://www.w3.org/2001/sw/BestPractices/WNET/DLP3941_daml.html))."@en ;
                                                                                          rdfs:label "participant place of"@en .


###  http://www.ontologydesignpatterns.org/ont/dlp/TemporalRelations.owl#follows
<http://www.ontologydesignpatterns.org/ont/dlp/TemporalRelations.owl#follows> rdf:type owl:ObjectProperty ;
                                                                              owl:inverseOf <http://www.ontologydesignpatterns.org/ont/dlp/TemporalRelations.owl#precedes> ;
                                                                              rdf:type owl:TransitiveProperty ;
                                                                              rdfs:domain <http://www.ontologydesignpatterns.org/ont/dlp/DOLCE-Lite.owl#perdurant> ;
                                                                              rdfs:range <http://www.ontologydesignpatterns.org/ont/dlp/DOLCE-Lite.owl#perdurant> ;
                                                                              rdfs:comment "In GOLEM, describes the temporal relation between two narrative events (G5) or psychological states (G3), either chronologically or causally."@en ,
                                                                                           "Temporal precedence between two perdurants. No further dependence is implied (e.g. mereological, causal) ([DOLCE-Lite-Plus, 2005](https://www.w3.org/2001/sw/BestPractices/WNET/DLP3941_daml.html))."@en ;
                                                                              rdfs:label "follows"@en ;
                                                                              skos:example "Ron argues with Hermione about her date (G5) follows Hermione arrives at the ball with Viktor Krum (G5)." ,
                                                                                           "Ron argues with Hermione about her date (G5) follows Ron has state “jealousy” (G3) during the Yule Ball (G5)." .


###  http://www.ontologydesignpatterns.org/ont/dlp/TemporalRelations.owl#precedes
<http://www.ontologydesignpatterns.org/ont/dlp/TemporalRelations.owl#precedes> rdf:type owl:ObjectProperty ,
                                                                                        owl:TransitiveProperty ;
                                                                               rdfs:domain <http://www.ontologydesignpatterns.org/ont/dlp/DOLCE-Lite.owl#perdurant> ;
                                                                               rdfs:range <http://www.ontologydesignpatterns.org/ont/dlp/DOLCE-Lite.owl#perdurant> ;
                                                                               rdfs:comment "In GOLEM, describes the temporal relation between two narrative events (G5) or psychological states (G3), either chronologically or causally." ,
                                                                                            "Temporal precedence between two perdurants. No further dependence is implied (e.g. mereological, causal) ([DOLCE-Lite-Plus, 2005](https://www.w3.org/2001/sw/BestPractices/WNET/DLP3941_daml.html))." ;
                                                                               rdfs:label "precedes"@en .


###  http://www.ontologydesignpatterns.org/ont/dlp/TemporalRelations.owl#temporal-location
<http://www.ontologydesignpatterns.org/ont/dlp/TemporalRelations.owl#temporal-location> rdf:type owl:ObjectProperty ;
                                                                                        owl:inverseOf <http://www.ontologydesignpatterns.org/ont/dlp/TemporalRelations.owl#temporal-location-of> ;
                                                                                        rdfs:domain <http://www.ontologydesignpatterns.org/ont/dlp/DOLCE-Lite.owl#perdurant> ;
                                                                                        rdfs:range <http://www.ontologydesignpatterns.org/ont/dlp/DOLCE-Lite.owl#region> ;
                                                                                        rdfs:comment "Analytical location holding between physical perdurants and temporal regions  ([DOLCE-Lite-Plus, 2005](https://www.w3.org/2001/sw/BestPractices/WNET/DLP3941_daml.html))." ,
                                                                                                     "In GOLEM, describes the specific time point at which a narrative event (G5) occurs." ;
                                                                                        rdfs:label "temporal location"@en ;
                                                                                        skos:example "The Yule Ball in *Harry Potter and the Goblet of Fire* (movie, 2005) (G5) has temporal location Christmas Eve (time-interval)." .


###  http://www.ontologydesignpatterns.org/ont/dlp/TemporalRelations.owl#temporal-location-of
<http://www.ontologydesignpatterns.org/ont/dlp/TemporalRelations.owl#temporal-location-of> rdf:type owl:ObjectProperty ;
                                                                                           rdfs:domain <http://www.ontologydesignpatterns.org/ont/dlp/DOLCE-Lite.owl#region> ;
                                                                                           rdfs:range <http://www.ontologydesignpatterns.org/ont/dlp/DOLCE-Lite.owl#perdurant> ;
                                                                                           rdfs:comment "Analytical location holding between physical perdurants and temporal regions  ([DOLCE-Lite-Plus, 2005](https://www.w3.org/2001/sw/BestPractices/WNET/DLP3941_daml.html))." ,
                                                                                                        "In GOLEM, describes the specific time point at which a narrative event (G5) occurs." ;
                                                                                           rdfs:label "temporal location of"@en .


###  http://www.ontologydesignpatterns.org/ont/dlp/TemporalRelations.owl#temporally-included-in
<http://www.ontologydesignpatterns.org/ont/dlp/TemporalRelations.owl#temporally-included-in> rdf:type owl:ObjectProperty ;
                                                                                             owl:inverseOf <http://www.ontologydesignpatterns.org/ont/dlp/TemporalRelations.owl#temporally-includes> ;
                                                                                             rdf:type owl:TransitiveProperty ;
                                                                                             rdfs:domain <http://www.ontologydesignpatterns.org/ont/dlp/DOLCE-Lite.owl#perdurant> ;
                                                                                             rdfs:range <http://www.ontologydesignpatterns.org/ont/dlp/DOLCE-Lite.owl#perdurant> ;
                                                                                             rdfs:comment "In GOLEM, indicates that a general event (G5) contains one or more sub-events (G5) or psychological states (G3)."@en ,
                                                                                                          "All temporal locations of perdurant x are also temporal locations of perdurant y  ([DOLCE-Lite-Plus, 2005](https://www.w3.org/2001/sw/BestPractices/WNET/DLP3941_daml.html))." ;
                                                                                             rdfs:label "temporally included in" .


###  http://www.ontologydesignpatterns.org/ont/dlp/TemporalRelations.owl#temporally-includes
<http://www.ontologydesignpatterns.org/ont/dlp/TemporalRelations.owl#temporally-includes> rdf:type owl:ObjectProperty ,
                                                                                                   owl:TransitiveProperty ;
                                                                                          rdfs:domain <http://www.ontologydesignpatterns.org/ont/dlp/DOLCE-Lite.owl#perdurant> ;
                                                                                          rdfs:range <http://www.ontologydesignpatterns.org/ont/dlp/DOLCE-Lite.owl#perdurant> ;
                                                                                          rdfs:comment "All temporal locations of perdurant x are also temporal locations of perdurant y  ([DOLCE-Lite-Plus, 2005](https://www.w3.org/2001/sw/BestPractices/WNET/DLP3941_daml.html))." ,
                                                                                                       "In GOLEM, indicates that a general event (G5) contains one or more sub-events (G5) or psychological states (G3)." ;
                                                                                          rdfs:label "temporally includes"@en ;
                                                                                          skos:example "The Battle of Hogwarts (G5) temporally includes the death of Voldemort (G5)." ,
                                                                                                       "The Yule Ball in Harry Potter and the Goblet of Fire (movie, 2005) (G5) temporally includes Ron's jealousy (G3)." .


###  http://www.ontologydesignpatterns.org/ont/dlp/TemporalRelations.owl#temporally-overlaps
<http://www.ontologydesignpatterns.org/ont/dlp/TemporalRelations.owl#temporally-overlaps> rdf:type owl:ObjectProperty ;
                                                                                          owl:inverseOf <http://www.ontologydesignpatterns.org/ont/dlp/TemporalRelations.owl#temporally-overlaps> ;
                                                                                          rdf:type owl:SymmetricProperty ;
                                                                                          rdfs:domain <http://www.ontologydesignpatterns.org/ont/dlp/DOLCE-Lite.owl#perdurant> ;
                                                                                          rdfs:range <http://www.ontologydesignpatterns.org/ont/dlp/DOLCE-Lite.owl#perdurant> ;
                                                                                          rdfs:comment "In GOLEM, indicates that two narrative events (G5) or psychological states (G3) overlap at some point in time." ,
                                                                                                       "Temporal overlap: having a (partly) common temporal location  ([DOLCE-Lite-Plus, 2005](https://www.w3.org/2001/sw/BestPractices/WNET/DLP3941_daml.html))." ;
                                                                                          rdfs:label "temporally overlaps"@en ;
                                                                                          skos:example "Ron’s jealousy (G3) temporally overlaps with Hermione’s arrival at the ball with Viktor Krum (G5)." .


###  http://www.w3.org/2000/01/rdf-schema#member
rdfs:member rdf:type owl:ObjectProperty ;
            rdfs:comment "A member of the subject resource." ,
                         "In GOLEM, describes the sequence or order of items within a (dlp:)course, like fabula (G7) or syuzhet (G8)." ;
            rdfs:isDefinedBy rdfs: ;
            rdfs:label "member" ;
            skos:example """The fabula of Battle of Hogwarts in Harry Potter and the Deathly Hallows orders events as follows:
rdf:_1 Voldemort casts the \"Avada Kedavra\" curse.
rdf:_2 Harry casts \"Expelliarmus\"
rdf:_3 The spells collide in midair, etc.""" .


###  https://ontology.golemlab.eu/GP0_has_feature
gc:GP0_has_feature rdf:type owl:ObjectProperty ;
                   owl:inverseOf gc:GP0i_is_feature_of ;
                   rdfs:domain <http://www.cidoc-crm.org/cidoc-crm/E70_Thing> ;
                   rdfs:range gc:G2_Feature ;
                   rdfs:comment "Indicates that a narrative or character has certain features." ;
                   rdfs:label "has feature" ;
                   skos:example "Harry Potter (G1) has feature bravery (G17)." ,
                                """The text of Harry Potter and the Deathly Hallows (J. K. Rowling, 2007) (F2) hasFeature third-person limited 
perspective (G18).""" .


###  https://ontology.golemlab.eu/GP0i_is_feature_of
gc:GP0i_is_feature_of rdf:type owl:ObjectProperty ;
                      rdfs:domain gc:G2_Feature ;
                      rdfs:range <http://www.cidoc-crm.org/cidoc-crm/E70_Thing> ;
                      rdfs:comment "Indicates that a narrative or character has certain features." ;
                      rdfs:label "is feature of" .


###  https://ontology.golemlab.eu/GP1_is_character_in
gc:GP1_is_character_in rdf:type owl:ObjectProperty ;
                       owl:inverseOf gc:GP1i_has_Character ;
                       rdfs:domain gc:G1_Character ;
                       rdfs:range <http://iflastandards.info/ns/lrm/lrmoo/F1_Work> ;
                       rdfs:comment "Indicates that a character appears in a work."@en ;
                       rdfs:label "is character in"@en ;
                       skos:example "Harry Potter (G1) *is character in* *Harry Potter and the Philosopher's Stone* (movie, 2001) (F1)." .


###  https://ontology.golemlab.eu/GP1i_has_Character
gc:GP1i_has_Character rdf:type owl:ObjectProperty ;
                      rdfs:domain <http://iflastandards.info/ns/lrm/lrmoo/F1_Work> ;
                      rdfs:range gc:G1_Character ;
                      rdfs:comment "Indicates that a character appears in a work." ;
                      rdfs:label "has character" .


#################################################################
#    Data properties
#################################################################

###  http://www.cidoc-crm.org/cidoc-crm/P90_has_value
<http://www.cidoc-crm.org/cidoc-crm/P90_has_value> rdf:type owl:DatatypeProperty ;
                                                   rdfs:domain <http://www.cidoc-crm.org/cidoc-crm/E54_Dimension> ;
                                                   rdfs:range rdfs:Literal ;
                                                   rdfs:comment "This property allows an instance of E54 Dimension to be approximated by an instance of E60 Number primitive." ;
                                                   rdfs:label "P90 has value" ;
                                                   skos:example """Kudos (E54) has value 59 (E60).
(Smile as Bright as the Sun as You Fade into Darkness from AO3)""" ,
                                                                "Word count (E54) has value 1,337 (E60)." .


#################################################################
#    Classes
#################################################################

###  http://iflastandards.info/ns/lrm/lrmoo/F1_Work
<http://iflastandards.info/ns/lrm/lrmoo/F1_Work> rdf:type owl:Class ;
                                                 rdfs:subClassOf <http://www.cidoc-crm.org/cidoc-crm/E89_Propositional_Object> ,
                                                                 <http://www.ontologydesignpatterns.org/ont/dlp/ExtendedDnS.owl#description> ,
                                                                 [ rdf:type owl:Restriction ;
                                                                   owl:onProperty <http://iflastandards.info/ns/lrm/lrmoo/R3_is_realised_in> ;
                                                                   owl:someValuesFrom <http://iflastandards.info/ns/lrm/lrmoo/F2_Expression>
                                                                 ] ,
                                                                 [ rdf:type owl:Restriction ;
                                                                   owl:onProperty <http://www.cidoc-crm.org/cidoc-crm/P130_shows_features_of> ;
                                                                   owl:someValuesFrom gc:G15_Fandom
                                                                 ] ,
                                                                 [ rdf:type owl:Restriction ;
                                                                   owl:onProperty <http://www.ontologydesignpatterns.org/ont/dlp/DOLCE-Lite.owl#proper-part> ;
                                                                   owl:someValuesFrom gc:G9_Narrative_Unit
                                                                 ] ,
                                                                 [ rdf:type owl:Restriction ;
                                                                   owl:onProperty <http://www.ontologydesignpatterns.org/ont/dlp/ExtendedDnS.owl#d-uses> ;
                                                                   owl:someValuesFrom gc:G7_Fabula
                                                                 ] ,
                                                                 [ rdf:type owl:Restriction ;
                                                                   owl:onProperty <http://www.ontologydesignpatterns.org/ont/dlp/ExtendedDnS.owl#d-uses> ;
                                                                   owl:someValuesFrom gc:G8_Syuzhet
                                                                 ] ,
                                                                 [ rdf:type owl:Restriction ;
                                                                   owl:onProperty <http://www.ontologydesignpatterns.org/ont/dlp/ExtendedDnS.owl#satisfied-by> ;
                                                                   owl:someValuesFrom gc:G12_Setting
                                                                 ] ;
                                                 rdfs:comment """Scope note:
This class comprises distinct intellectual ideas conveyed in artistic and intellectual creations, such a poems, stories or musical compositions.
A Work is the outcome of an intellectual process of one or more persons. Inherent to the notion of work is the existence of recognisable realizations of the work in the form of one or more expressions. Works are often regarded as finished and discrete e.g. when declared as such by the creator of the work or based on the elaboration or logical coherence of its content. However, works may be recognized as existing but unfinished e.g. if the creators deliberately or accidentally never explicitly finished a particular Expression but have left behind partial expressions.
In the absence of explicit information about the initial conception, which is rarely available, the first expression created constitutes witness of the beginning of existence of a Work.
A Work can evolve over time, such as through revised editions. A Work may be elaborated by one or more Actors simultaneously, in parallel, or over time. Additional expressions of a Work can continue to be created over time.
The boundaries of a Work have nothing to do with the value of the intellectual achievement but only with the dominance of a concept.
The main purpose of this class is to enable bringing together intellectually equivalent Expressions in order to display to a user all available alternatives of the same intellectual or artistic content  ([LRMoo version1.0, 2024](https://www.cidoc-crm.org/extensions/lrmoo/html/LRMoo_v1.0.html))."""@en ,
                                                              "“A Work is the outcome of an intellectual process of one or more persons. Inherent to the notion of work is the existence of recognisable realizations of the work in the form of one or more expressions.”. A Work is a specific variant of a narrative Stoff. It includes specific characters, events, themes, and settings that are organized in a particular way (e.g. syuzhet)."@en ;
                                                 rdfs:label "F1 Work"@en ;
                                                 skos:example "*Harry Potter and the Philosopher's Stone* (movie, 2001)." .


###  http://iflastandards.info/ns/lrm/lrmoo/F2_Expression
<http://iflastandards.info/ns/lrm/lrmoo/F2_Expression> rdf:type owl:Class ;
                                                       rdfs:subClassOf <http://www.cidoc-crm.org/cidoc-crm/E73_Information_Object> ,
                                                                       [ rdf:type owl:Restriction ;
                                                                         owl:onProperty <http://iflastandards.info/ns/lrm/lrmoo/R3i_realises> ;
                                                                         owl:someValuesFrom <http://iflastandards.info/ns/lrm/lrmoo/F1_Work>
                                                                       ] ,
                                                                       [ rdf:type owl:Restriction ;
                                                                         owl:onProperty <http://iflastandards.info/ns/lrm/lrmoo/R5_has_component> ;
                                                                         owl:someValuesFrom <http://iflastandards.info/ns/lrm/lrmoo/F2_Expression>
                                                                       ] ,
                                                                       [ rdf:type owl:Restriction ;
                                                                         owl:onProperty <http://www.cidoc-crm.org/cidoc-crm/P16i_was_used_for> ;
                                                                         owl:someValuesFrom <http://www.cidoc-crm.org/cidoc-crm/E13_Attribute_Assignment>
                                                                       ] ;
                                                       rdfs:comment """Scope note:
This class comprises the intellectual or artistic realisations of Works in the form of identifiable immaterial objects, such as texts, poems, jokes, musical or choreographic notations, movement pattern, sound pattern, images, multimedia objects, or any combination of such forms. The substance of F2 Expression is signs.
An Expression is the outcome of the intellectual or creative process of realizing a Work. Subsequent expressions conveying the same work may be created over time.
Expressions do not depend on a specific physical carrier and can exist on one or more carriers simultaneously. As far as bibliographic practice is concerned, only instances of F2 Expression that are externalised on physical carriers other than both the creator’s brain and an auditor’s brain are taken into account.
The form of F2 Expression is an inherent characteristic of the F2 Expression. Differences in form imply different Expressions (e.g., from text to spoken word, a transcript of a recording). Similarly, differences in language or means of performance imply different Expressions (e.g., translations or arrangements for different instruments). Thus, if a text is revised or modified, the result is considered to be a new F2 Expression. While theoretically any change in signs will result in a new Expression, conventionally the context and use will determine the rules for distinguishing among expressions.
An instance of F2 Expression which includes spoken or written text may be multiply instantiated as an instance of E33 Linguistic Object. This allows for the association of the E56 Language of the text with the instance of F2 Expression by using the property P72 has language (is language of) ([LRMoo version1.0, 2024](https://www.cidoc-crm.org/extensions/lrmoo/html/LRMoo_v1.0.html))."""@en ,
                                                                    "In GOLEM, an expression is the realization of a work, reflecting how a story is conveyed through specific forms such as texts, audio, movies, or other visual media." ;
                                                       rdfs:label "F2 Expression"@en ;
                                                       skos:example "The text of the English version of *Harry Potter and the Philosopher's Stone*." .


###  http://www.cidoc-crm.org/cidoc-crm/E13_Attribute_Assignment
<http://www.cidoc-crm.org/cidoc-crm/E13_Attribute_Assignment> rdf:type owl:Class ;
                                                              rdfs:subClassOf <http://www.cidoc-crm.org/cidoc-crm/E7_Activity> ,
                                                                              [ rdf:type owl:Restriction ;
                                                                                owl:onProperty <http://www.cidoc-crm.org/cidoc-crm/P140_assigned_attribute_to> ;
                                                                                owl:someValuesFrom <http://www.cidoc-crm.org/cidoc-crm/E1_CRM_Entity>
                                                                              ] ,
                                                                              [ rdf:type owl:Restriction ;
                                                                                owl:onProperty <http://www.cidoc-crm.org/cidoc-crm/P141_assigned> ;
                                                                                owl:someValuesFrom <http://www.cidoc-crm.org/cidoc-crm/E1_CRM_Entity>
                                                                              ] ,
                                                                              [ rdf:type owl:Restriction ;
                                                                                owl:onProperty <http://www.cidoc-crm.org/cidoc-crm/P177_assigned_property_of_type> ;
                                                                                owl:someValuesFrom <http://www.cidoc-crm.org/cidoc-crm/E55_Type>
                                                                              ] ;
                                                              rdfs:comment """This class comprises the actions of making assertions about one property of an object or any single relation between two items or concepts. The type of the property asserted to hold between two items or concepts can be described by the property P177 assigned property of type (is type of property assigned): E55 Type.
For example, the class describes the actions of people making propositions and statements during certain scientific/scholarly procedures, e.g. the person and date when a condition statement was made, an identifier was assigned, the museum object was measured, etc. Which kinds of such assignments and statements need to be documented explicitly in structures of a schema rather than free text, depends on whether this information should be accessible by structured queries.
This class allows for the documentation of how the respective assignment came about, and whose opinion it was. Note that all instances of properties described in a knowledge base are the opinion of someone. Per default, they are the opinion of the team maintaining the knowledge base. This fact must not individually be registered for all instances of properties provided by the maintaining team, because it would result in an endless recursion of whose opinion was the description of an opinion. Therefore, the use of instances of E13 Attribute Assignment marks the fact that the maintaining team is in general neutral to the validity of the respective assertion, but registers someone else’s opinion and how it came about.
All properties assigned in such an action can also be seen as directly relating the respective pair of items or concepts. Multiple use of instances of E13 Attribute Assignment may possibly lead to a collection of contradictory values ([CIDOC-CRM version 7.1.3, 2024](https://cidoc-crm.org/html/cidoc_crm_v7.1.3.html))."""@en ,
                                                                           "In GOLEM, an attribute assignment is a framework for modeling observations and inference-making processes. It involves the act of assigning a property to an entity or asserting a relationship between concepts. It is the activity of making a statement that links an attribute to a subject." ;
                                                              rdfs:label "E13 Attribute Assignment"@en ;
                                                              skos:example "Assigning the topic “friendship” to the work Harry Potter and the Philosopher's Stone." .


###  http://www.cidoc-crm.org/cidoc-crm/E1_CRM_Entity
<http://www.cidoc-crm.org/cidoc-crm/E1_CRM_Entity> rdf:type owl:Class ;
                                                   owl:equivalentClass <http://www.ontologydesignpatterns.org/ont/dlp/DOLCE-Lite.owl#particular> ;
                                                   rdfs:comment "This class comprises all things in the universe of discourse of the CIDOC Conceptual Reference Model. It is an abstract concept providing for three general properties: Identification by name or appellation, and in particular by a preferred identifier Classification by type, allowing further refinement of the specific subclass to which an instance belongs Attachment of free text and other unstructured data for the expression of anything not captured by formal properties. All other classes within the CIDOC CRM are directly or indirectly specialisations of E1 CRM Entity ([CIDOC-CRM version 7.1.3, 2024](https://cidoc-crm.org/html/cidoc_crm_v7.1.3.html))."@en ;
                                                   rdfs:label "E1 CRM Entity"@en .


###  http://www.cidoc-crm.org/cidoc-crm/E28_Conceptual_Object
<http://www.cidoc-crm.org/cidoc-crm/E28_Conceptual_Object> rdf:type owl:Class ;
                                                           rdfs:comment """This class comprises non-material products of our minds and other human produced data that have become objects of a discourse about their identity, circumstances of creation, or historical implication. The production of such information might have been supported by the use of technical devices such as cameras or computers.
Characteristically, instances of this class are created, invented or thought by someone, and then may be documented or communicated between persons. Instances of E28 Conceptual Object have the ability to exist on more than one particular carrier at the same time, such as paper, electronic signals, marks, audio media, paintings, photos, human memories, etc.
They cannot be destroyed. They exist as long as they can be found on at least one carrier or in at least one human memory. Their existence ends when the last carrier and the last memory are lost ([CIDOC-CRM version 7.1.3, 2024](https://cidoc-crm.org/html/cidoc_crm_v7.1.3.html))."""@en ;
                                                           rdfs:label "E28 Conceptual Object"@en .


###  http://www.cidoc-crm.org/cidoc-crm/E54_Dimension
<http://www.cidoc-crm.org/cidoc-crm/E54_Dimension> rdf:type owl:Class ;
                                                   rdfs:subClassOf <http://www.cidoc-crm.org/cidoc-crm/E1_CRM_Entity> ;
                                                   rdfs:comment """This class comprises quantifiable properties that can be measured by some calibrated means and can be approximated by values, i.e. points or regions in a mathematical or conceptual space, such as natural or real numbers, RGB values, etc.
An instance of E54 Dimension represents the empirical or theoretically derived quantity, including the precision tolerances resulting from the particular method or calculation. The identity of an instance of E54 Dimension depends on the method of its determination because each method may produce different values even when determining comparable qualities. For instance, the wingspan of a bird alive or dead is a different dimension. Thermoluminescence dating and Rehydroxylation [RHX] dating are different dimensions of temporal distance from now, even if they aim at dating the same object. The method of determination should be expressed using the property P2 has type (is type of). Note that simple terms such as “diameter” or “length” are normally insufficient to unambiguously describe a respective dimension. In contrast, “maximum linear extent” may be sufficient.
The properties of the class E54 Dimension allow for expressing the numerical approximation of the values of instances of E54 Dimension adequate to the precision of the applied method of determination. If the respective quantity belongs to a non-discrete space according to the laws of physics, such as spatial distances, it is recommended to record them as approximations by intervals or regions of indeterminacy enclosing the assumed true values. For instance, a length of 5 cm may be recorded as 4.5-5.5 cm, according to the precision of the respective observation. Note, that comparability of values described in different units depends critically on the representation as value regions.
Numerical approximations in archaic instances of E58 Measurement Unit used in historical records should be preserved. Equivalents corresponding to current knowledge should be recorded as additional instances of E54 Dimension, as appropriate ([CIDOC-CRM version 7.1.3, 2024](https://cidoc-crm.org/html/cidoc_crm_v7.1.3.html))."""@en ;
                                                   rdfs:label "E54 Dimension"@en ;
                                                   skos:example "The word count and kudos on AO3." .


###  http://www.cidoc-crm.org/cidoc-crm/E55_Type
<http://www.cidoc-crm.org/cidoc-crm/E55_Type> rdf:type owl:Class ;
                                              rdfs:subClassOf [ rdf:type owl:Restriction ;
                                                                owl:onProperty <http://www.cidoc-crm.org/cidoc-crm/P127_has_broader_term> ;
                                                                owl:someValuesFrom <http://www.cidoc-crm.org/cidoc-crm/E55_Type>
                                                              ] ,
                                                              [ rdf:type owl:Restriction ;
                                                                owl:onProperty <http://www.cidoc-crm.org/cidoc-crm/P127i_has_narrower_term> ;
                                                                owl:someValuesFrom <http://www.cidoc-crm.org/cidoc-crm/E55_Type>
                                                              ] ,
                                                              [ rdf:type owl:Restriction ;
                                                                owl:onProperty <http://www.cidoc-crm.org/cidoc-crm/P2i_is_type_of> ;
                                                                owl:someValuesFrom <http://www.cidoc-crm.org/cidoc-crm/E1_CRM_Entity>
                                                              ] ;
                                              rdfs:comment """This class comprises concepts denoted by terms from thesauri and controlled vocabularies used to characterize and classify instances of CIDOC CRM classes. Instances of E55 Type represent concepts, in contrast to instances of E41 Appellation which are used to name instances of CIDOC CRM classes.
E55 Type provides an interface to domain specific ontologies and thesauri. These can be represented in the CIDOC CRM as subclasses of E55 Type, forming hierarchies of terms, i.e. instances of E55 Type linked via P127 has broader term (has narrower term): E55 Type. Such hierarchies may be extended with additional properties ([CIDOC-CRM version 7.1.3, 2024](https://cidoc-crm.org/html/cidoc_crm_v7.1.3.html))."""@en ;
                                              rdfs:label "E55 Type"@en ;
                                              skos:example "The Tag categories on AO3, e.g. character tag or relationship tag." .


###  http://www.cidoc-crm.org/cidoc-crm/E58_Measurement_Unit
<http://www.cidoc-crm.org/cidoc-crm/E58_Measurement_Unit> rdf:type owl:Class ;
                                                          rdfs:comment """This class is a specialization of E55 Type and comprises the types of measurement units: feet, inches, centimetres, litres, lumens, etc.

This type is used categorically in the model without reference to instances of it, i.e. the model does not foresee the description of instances of instances of E58 Measurement Unit, e.g. “instances of cm”.

Système International (SI) units or internationally recognized non-SI terms should be used whenever possible, such as those defined by ISO80000:2009. Archaic Measurement Units used in historical records should be preserved.""" ;
                                                          rdfs:label "E58 Measurement Unit" ;
                                                          skos:example "word counts, kudos." .


###  http://www.cidoc-crm.org/cidoc-crm/E70_Thing
<http://www.cidoc-crm.org/cidoc-crm/E70_Thing> rdf:type owl:Class ;
                                               rdfs:comment """This general class comprises discrete, identifiable, instances of E77 Persistent Item that are documented as single units, that either consist of matter or depend on being carried by matter and are characterized by relative stability.
They may be intellectual products or physical things. They may, for instance, have a solid physical form, an electronic encoding, or they may be a logical concept or structure ([CIDOC-CRM version 7.1.3, 2024](https://cidoc-crm.org/html/cidoc_crm_v7.1.3.html))."""@en ;
                                               rdfs:label "E70 Thing"@en .


###  http://www.cidoc-crm.org/cidoc-crm/E73_Information_Object
<http://www.cidoc-crm.org/cidoc-crm/E73_Information_Object> rdf:type owl:Class ;
                                                            rdfs:comment """This class comprises identifiable immaterial items, such as poems, jokes, data sets, images, texts, multimedia objects, procedural prescriptions, computer program code, algorithm or mathematical formulae, that have an objectively recognizable structure and are documented as single units. The encoding structure known as a “named graph” also falls under this class, so that each “named graph” is an instance of E73 Information Object.
An instance of E73 Information Object does not depend on a specific physical carrier, which can include human memory, and it can exist on one or more carriers simultaneously.
Instances of E73 Information Object of a linguistic nature should be declared as instances of the E33 Linguistic Object subclass. Instances of E73 Information Object of a documentary nature should be declared as instances of the E31 Document subclass. Conceptual items such as types and classes are not instances of E73 Information Object, nor are ideas without a reproducible expression ([CIDOC-CRM version 7.1.3, 2024](https://cidoc-crm.org/html/cidoc_crm_v7.1.3.html))."""@en ;
                                                            rdfs:label "E73 Information Object"@en .


###  http://www.cidoc-crm.org/cidoc-crm/E7_Activity
<http://www.cidoc-crm.org/cidoc-crm/E7_Activity> rdf:type owl:Class ;
                                                 rdfs:comment """This class comprises actions intentionally carried out by instances of E39 Actor that result in changes of state in the cultural, social, or physical systems documented.
This notion includes complex, composite, and long-lasting actions such as the building of a settlement or a war, as well as simple, short-lived actions such as the opening of a door ([CIDOC-CRM version 7.1.3, 2024](https://cidoc-crm.org/html/cidoc_crm_v7.1.3.html))."""@en ;
                                                 rdfs:label "E7 Activity"@en .


###  http://www.cidoc-crm.org/cidoc-crm/E89_Propositional_Object
<http://www.cidoc-crm.org/cidoc-crm/E89_Propositional_Object> rdf:type owl:Class ;
                                                              rdfs:comment """This class comprises immaterial items, including but not limited to stories, plots, procedural prescriptions, algorithms, laws of physics or images that are, or represent in some sense, sets of propositions about real or imaginary things and that are documented as single units or serve as topic of discourse.
This class also comprises items that are “about” something in the sense of a subject. In the wider sense, this class includes expressions of psychological value such as non-figural art and musical themes. However, conceptual items such as types and classes are not instances of E89 Propositional Object. This should not be confused with the definition of a type, which is indeed an instance of E89 Propositional Object ([CIDOC-CRM version 7.1.3, 2024](https://cidoc-crm.org/html/cidoc_crm_v7.1.3.html))."""@en ;
                                                              rdfs:label "E89 Propositional Object"@en .


###  http://www.loa-cnr.it/ontologies/CommonSenseMapping.owl#geographical-place
<http://www.loa-cnr.it/ontologies/CommonSenseMapping.owl#geographical-place> rdf:type owl:Class ;
                                                                             rdfs:subClassOf <http://www.ontologydesignpatterns.org/ont/dlp/CommonSenseMapping.owl#non-physical-place> ,
                                                                                             [ rdf:type owl:Restriction ;
                                                                                               owl:onProperty <http://www.ontologydesignpatterns.org/ont/dlp/DOLCE-Lite.owl#generic-dependent> ;
                                                                                               owl:someValuesFrom gc:G13_Narrative_Location
                                                                                             ] ;
                                                                             owl:disjointWith <http://www.loa-cnr.it/ontologies/ExtendedDnS.owl#social-relationship> ,
                                                                                              <http://www.ontologydesignpatterns.org/ont/dlp/ExtendedDnS.owl#course> ,
                                                                                              <http://www.ontologydesignpatterns.org/ont/dlp/ExtendedDnS.owl#description> ,
                                                                                              <http://www.ontologydesignpatterns.org/ont/dlp/ExtendedDnS.owl#role> ,
                                                                                              <http://www.ontologydesignpatterns.org/ont/dlp/ExtendedDnS.owl#situation> ,
                                                                                              gc:G10_Narrative_Function ,
                                                                                              gc:G11_Narrative_Role ,
                                                                                              gc:G12_Setting ,
                                                                                              gc:G14_Narrative-Stoff ,
                                                                                              gc:G4_Social_Relationship ,
                                                                                              gc:G6_Relationship_Role ,
                                                                                              gc:G7_Fabula ,
                                                                                              gc:G8_Syuzhet ,
                                                                                              gc:G9_Narrative_Unit ;
                                                                             rdfs:comment "A non-physical place, generically dependent on some (physical) geographical object ([DOLCE-Lite-Plus, 2005](https://www.w3.org/2001/sw/BestPractices/WNET/DLP3941_daml.html))." ;
                                                                             rdfs:label "Geographical place" .


###  http://www.loa-cnr.it/ontologies/ExtendedDnS.owl#social-relationship
<http://www.loa-cnr.it/ontologies/ExtendedDnS.owl#social-relationship> rdf:type owl:Class ;
                                                                       rdfs:subClassOf [ rdf:type owl:Restriction ;
                                                                                         owl:onProperty <http://www.ontologydesignpatterns.org/ont/dlp/ExtendedDnS.owl#involves> ;
                                                                                         owl:minCardinality "2"^^xsd:nonNegativeInteger
                                                                                       ] ;
                                                                       owl:disjointWith <http://www.ontologydesignpatterns.org/ont/dlp/CommonSenseMapping.owl#non-physical-place> ,
                                                                                        <http://www.ontologydesignpatterns.org/ont/dlp/ExtendedDnS.owl#agentive-social-object> ,
                                                                                        <http://www.ontologydesignpatterns.org/ont/dlp/ExtendedDnS.owl#course> ,
                                                                                        <http://www.ontologydesignpatterns.org/ont/dlp/ExtendedDnS.owl#role> ,
                                                                                        <http://www.ontologydesignpatterns.org/ont/dlp/ExtendedDnS.owl#situation> ,
                                                                                        gc:G10_Narrative_Function ,
                                                                                        gc:G11_Narrative_Role ,
                                                                                        gc:G12_Setting ,
                                                                                        gc:G13_Narrative_Location ,
                                                                                        gc:G1_Character ,
                                                                                        gc:G6_Relationship_Role ,
                                                                                        gc:G7_Fabula ,
                                                                                        gc:G8_Syuzhet ;
                                                                       rdfs:comment "A social description defining roles for the interaction of rational agents  ([DOLCE-Lite-Plus, 2005](https://www.w3.org/2001/sw/BestPractices/WNET/DLP3941_daml.html))." ;
                                                                       rdfs:label "social relationship" .


###  http://www.ontologydesignpatterns.org/ont/dlp/CommonSenseMapping.owl#non-physical-place
<http://www.ontologydesignpatterns.org/ont/dlp/CommonSenseMapping.owl#non-physical-place> rdf:type owl:Class ;
                                                                                          owl:disjointWith <http://www.ontologydesignpatterns.org/ont/dlp/ExtendedDnS.owl#course> ,
                                                                                                           <http://www.ontologydesignpatterns.org/ont/dlp/ExtendedDnS.owl#description> ,
                                                                                                           <http://www.ontologydesignpatterns.org/ont/dlp/ExtendedDnS.owl#role> ,
                                                                                                           <http://www.ontologydesignpatterns.org/ont/dlp/ExtendedDnS.owl#situation> ,
                                                                                                           gc:G10_Narrative_Function ,
                                                                                                           gc:G11_Narrative_Role ,
                                                                                                           gc:G12_Setting ,
                                                                                                           gc:G14_Narrative-Stoff ,
                                                                                                           gc:G4_Social_Relationship ,
                                                                                                           gc:G6_Relationship_Role ,
                                                                                                           gc:G7_Fabula ,
                                                                                                           gc:G8_Syuzhet ,
                                                                                                           gc:G9_Narrative_Unit ;
                                                                                          rdfs:comment "A figure (e.g. Italy) for non-physical (i.e. socially- or cognitively-constructed) places. Non-physical places generically depend on physical places  ([DOLCE-Lite-Plus, 2005](https://www.w3.org/2001/sw/BestPractices/WNET/DLP3941_daml.html))."@en ;
                                                                                          rdfs:label "non physical place" .


###  http://www.ontologydesignpatterns.org/ont/dlp/DOLCE-Lite.owl#endurant
<http://www.ontologydesignpatterns.org/ont/dlp/DOLCE-Lite.owl#endurant> rdf:type owl:Class ;
                                                                        rdfs:comment "The main characteristic of endurants is that all of them are independent essential wholes. This does not mean that the corresponding property (being an endurant) carries proper unity, since there is no common unity criterion for endurants. Endurants can 'genuinely' change in time, in the sense that the very same endurant as a whole can have incompatible properties at different times. To see this, suppose that an endurant say 'this paper' has a property at a time t 'it's white', and a different, incompatible property at time t' 'it's yellow': in both cases we refer to the whole object, without picking up any particular part of it. Within endurants, we distinguish between physical and non-physical endurants, according to whether they have direct spatial qualities. Within physical endurants, we distinguish between amounts of matter, objects, and features  ([DOLCE-Lite-Plus, 2005](https://www.w3.org/2001/sw/BestPractices/WNET/DLP3941_daml.html))."@en ;
                                                                        rdfs:label "endurant"@en .


###  http://www.ontologydesignpatterns.org/ont/dlp/DOLCE-Lite.owl#particular
<http://www.ontologydesignpatterns.org/ont/dlp/DOLCE-Lite.owl#particular> rdf:type owl:Class ;
                                                                          rdfs:comment "AKA 'entity'. Any individual in the DOLCE domain of discourse. The extensional coverage of DOLCE is as large as possible, since it ranges on 'possibilia', i.e all possible individuals that can be postulated by means of DOLCE axioms. Possibilia include physical objects, substances, processes, qualities, conceptual regions, non-physical objects, collections and even arbitrary sums of objects. Extensions of DOLCE included in this ontology also feature 'situations' (qualified reifications of states of affairs)  ([DOLCE-Lite-Plus, 2005](https://www.w3.org/2001/sw/BestPractices/WNET/DLP3941_daml.html))."@en ;
                                                                          rdfs:label "particular"@en .


###  http://www.ontologydesignpatterns.org/ont/dlp/DOLCE-Lite.owl#perdurant
<http://www.ontologydesignpatterns.org/ont/dlp/DOLCE-Lite.owl#perdurant> rdf:type owl:Class ;
                                                                         rdfs:comment "Perdurants (AKA occurrences) comprise what are variously called events, processes, phenomena, activities and states. They can have temporal parts or spatial parts. For instance, the first movement of (an execution of) a symphony is a temporal part of it. On the other side, the play performed by the left side of the orchestra is a spatial part. In both cases, these parts are occurrences themselves. We assume that objects cannot be parts of occurrences, but rather they participate in them. Perdurants extend in time by accumulating different temporal parts, so that, at any time they are present, they are only partially present, in the sense that some of their proper temporal parts (e.g., their previous or future phases) may be not present. E.g., the piece of paper you are reading now is wholly present, while some temporal parts of your reading are not present any more. Philosophers say that endurants are entities that are in time, while lacking however temporal parts (so to speak, all their parts flow with them in time). Perdurants, on the other hand, are entities that happen in time, and can have temporal parts (all their parts are fixed in time)  ([DOLCE-Lite-Plus, 2005](https://www.w3.org/2001/sw/BestPractices/WNET/DLP3941_daml.html))."@en ;
                                                                         rdfs:label "perdurant"@en .


###  http://www.ontologydesignpatterns.org/ont/dlp/DOLCE-Lite.owl#region
<http://www.ontologydesignpatterns.org/ont/dlp/DOLCE-Lite.owl#region> rdf:type owl:Class ;
                                                                      rdfs:comment "We distinguish between a quality (e.g., the color of a specific rose), and its value (e.g., a particular shade of red). The latter is called quale, and describes the position of an individual quality within a certain conceptual space (called here quality space) Gardenfors (2000). So when we say that two roses have (exactly) the same color, we mean that their color qualities, which are distinct, have the same position in the color space, that is they have the same color quale  ([DOLCE-Lite-Plus, 2005](https://www.w3.org/2001/sw/BestPractices/WNET/DLP3941_daml.html))."@en ;
                                                                      rdfs:label "region"@en .


###  http://www.ontologydesignpatterns.org/ont/dlp/DOLCE-Lite.owl#state
<http://www.ontologydesignpatterns.org/ont/dlp/DOLCE-Lite.owl#state> rdf:type owl:Class ;
                                                                     rdfs:comment "Within stative occurrences, we distinguish between states and processes according to homeomericity: sitting is classified as a state but running is classified as a process, since there are (very short) temporal parts of a running that are not themselves runnings. In general, states differ from situations because they are not assumed to have a description from which they depend. They can be sequenced by some course, but they do not require a description as a unifying criterion. On the other hand, at any time, one can conceive a description that asserts the constraints by which a state of a certian type is such, and in this case, it becomes a situation. Since the decision of designing an explicit description that unifies a perdurant depends on context, task, interest, application, etc., when aligning an ontology do DLP, there can be indecision on where to align a state-oriented class. For example, in the WordNet alignment, we have decided to put only some physical states under 'state', e.g. 'turgor', in order to stress the social orientedness of DLP. But whereas we need to talk explicitly of the criteria by which we conceive turgor states, these will be put under 'situation'. Similar considerations are made for the other types of perdurants in DOLCE. A different notion of event (dealing with change) is currently investigated for further developments: being 'achievement', 'accomplishment', 'state', 'event', etc. can be also considered 'aspects' of processes or of parts of them. For example, the same process 'rock erosion in the Sinni valley' can be conceptualized as an accomplishment (what has brought the current state that e.g. we are trying to explain), as an achievement (the erosion process as the result of a previous accomplishment), as a state (if we collapse the time interval of the erosion into a time point), or as an event (what has changed our focus from a state to another). In the erosion case, we could have good motivations to shift from one aspect to another: a) causation focus, b) effectual focus, c) condensation d) transition (causality). If we want to consider all the aspects of a process together, we need to postulate a unifying descriptive set of criteria (i.e. a 'description'), according to which that process is circumstantiated in a 'situation'. The different aspects will arise as a parts of a same situation  ([DOLCE-Lite-Plus, 2005](https://www.w3.org/2001/sw/BestPractices/WNET/DLP3941_daml.html))."@en ;
                                                                     rdfs:label "state"@en .


###  http://www.ontologydesignpatterns.org/ont/dlp/DOLCE-Lite.owl#time-interval
<http://www.ontologydesignpatterns.org/ont/dlp/DOLCE-Lite.owl#time-interval> rdf:type owl:Class ;
                                                                             rdfs:subClassOf [ rdf:type owl:Restriction ;
                                                                                               owl:onProperty <http://www.ontologydesignpatterns.org/ont/dlp/ExtendedDnS.owl#setting> ;
                                                                                               owl:someValuesFrom gc:G12_Setting
                                                                                             ] ,
                                                                                             [ rdf:type owl:Restriction ;
                                                                                               owl:onProperty <http://www.ontologydesignpatterns.org/ont/dlp/TemporalRelations.owl#temporal-location-of> ;
                                                                                               owl:someValuesFrom gc:G5_Narrative_Event
                                                                                             ] ;
                                                                             rdfs:comment """A temporal region, measured according to a calendar
([DOLCE-Lite-Plus, 2005](https://www.w3.org/2001/sw/BestPractices/WNET/DLP3941_daml.html)).""" ,
                                                                                          "A time-interval or time-span in a narrative refers to a duration or a specific time point during which events take place. It encompasses the beginning, end, and the length of time between them, allowing for the placement of actions on a chronological timeline. It can represent broad periods, like an era, or specific moments, like a single date or time." ;
                                                                             rdfs:label "Time Interval" ;
                                                                             skos:example "July 31, 1980 (Harry Potter's birthday)" .


###  http://www.ontologydesignpatterns.org/ont/dlp/ExtendedDnS.owl#agentive-social-object
<http://www.ontologydesignpatterns.org/ont/dlp/ExtendedDnS.owl#agentive-social-object> rdf:type owl:Class ;
                                                                                       owl:disjointWith <http://www.ontologydesignpatterns.org/ont/dlp/ExtendedDnS.owl#course> ,
                                                                                                        <http://www.ontologydesignpatterns.org/ont/dlp/ExtendedDnS.owl#description> ,
                                                                                                        <http://www.ontologydesignpatterns.org/ont/dlp/ExtendedDnS.owl#role> ,
                                                                                                        gc:G10_Narrative_Function ,
                                                                                                        gc:G11_Narrative_Role ,
                                                                                                        gc:G14_Narrative-Stoff ,
                                                                                                        gc:G4_Social_Relationship ,
                                                                                                        gc:G6_Relationship_Role ,
                                                                                                        gc:G7_Fabula ,
                                                                                                        gc:G8_Syuzhet ,
                                                                                                        gc:G9_Narrative_Unit ;
                                                                                       rdfs:comment "A social object that is assumed to internally represent a plan. Since social objects are dependent on physical ones, it is not trivial to interpret the local sense in which a social object 'internally represents' a plan. For example, an institution can have the plan to promote or regulate some activities, but this is possible by means of the powers conferred to it by some legal system, through its representatives, and that plan has to be executed by means of the physical agents that 'act for' the institution ([DOLCE-Lite-Plus, 2005](https://www.w3.org/2001/sw/BestPractices/WNET/DLP3941_daml.html))."@en ;
                                                                                       rdfs:label "agentive social object"@en .


###  http://www.ontologydesignpatterns.org/ont/dlp/ExtendedDnS.owl#concept
<http://www.ontologydesignpatterns.org/ont/dlp/ExtendedDnS.owl#concept> rdf:type owl:Class ;
                                                                        rdfs:comment "AKA C-Description. A non-physical object that is defined by a description s, and whose function is classifying entities from a ground ontology in order to build situations that can satisfy s  ([DOLCE-Lite-Plus, 2005](https://www.w3.org/2001/sw/BestPractices/WNET/DLP3941_daml.html))." ;
                                                                        rdfs:label "concept"@en .


###  http://www.ontologydesignpatterns.org/ont/dlp/ExtendedDnS.owl#course
<http://www.ontologydesignpatterns.org/ont/dlp/ExtendedDnS.owl#course> rdf:type owl:Class ;
                                                                       owl:disjointWith <http://www.ontologydesignpatterns.org/ont/dlp/ExtendedDnS.owl#description> ,
                                                                                        <http://www.ontologydesignpatterns.org/ont/dlp/ExtendedDnS.owl#role> ,
                                                                                        <http://www.ontologydesignpatterns.org/ont/dlp/ExtendedDnS.owl#situation> ,
                                                                                        gc:G10_Narrative_Function ,
                                                                                        gc:G11_Narrative_Role ,
                                                                                        gc:G12_Setting ,
                                                                                        gc:G13_Narrative_Location ,
                                                                                        gc:G14_Narrative-Stoff ,
                                                                                        gc:G1_Character ,
                                                                                        gc:G4_Social_Relationship ,
                                                                                        gc:G6_Relationship_Role ,
                                                                                        gc:G9_Narrative_Unit ;
                                                                       rdfs:comment "A concept that classifies (in particular, it 'sequences') perdurants (processes, events, or states), as a component of some description. Courses are the descriptive counterpart of perdurants, and, since perdurants have endurants as participants, they are usually the function of some role  ([DOLCE-Lite-Plus, 2005](https://www.w3.org/2001/sw/BestPractices/WNET/DLP3941_daml.html))."@en ;
                                                                       rdfs:label "course"@en .


###  http://www.ontologydesignpatterns.org/ont/dlp/ExtendedDnS.owl#description
<http://www.ontologydesignpatterns.org/ont/dlp/ExtendedDnS.owl#description> rdf:type owl:Class ;
                                                                            owl:disjointWith <http://www.ontologydesignpatterns.org/ont/dlp/ExtendedDnS.owl#role> ,
                                                                                             <http://www.ontologydesignpatterns.org/ont/dlp/ExtendedDnS.owl#situation> ,
                                                                                             gc:G10_Narrative_Function ,
                                                                                             gc:G11_Narrative_Role ,
                                                                                             gc:G12_Setting ,
                                                                                             gc:G13_Narrative_Location ,
                                                                                             gc:G1_Character ,
                                                                                             gc:G6_Relationship_Role ,
                                                                                             gc:G7_Fabula ,
                                                                                             gc:G8_Syuzhet ;
                                                                            rdfs:comment "A description is a social object which represents a conceptualization (e.g. a mental object or state), hence it is generically dependent on some agent and communicable. Descriptions define or use concepts or figures, are expressed by an information object and can be satisfied by situations. The typology of descriptions is still preliminary  ([DOLCE-Lite-Plus, 2005](https://www.w3.org/2001/sw/BestPractices/WNET/DLP3941_daml.html))."@en ;
                                                                            rdfs:label "description"@en .


###  http://www.ontologydesignpatterns.org/ont/dlp/ExtendedDnS.owl#role
<http://www.ontologydesignpatterns.org/ont/dlp/ExtendedDnS.owl#role> rdf:type owl:Class ;
                                                                     owl:disjointWith <http://www.ontologydesignpatterns.org/ont/dlp/ExtendedDnS.owl#situation> ,
                                                                                      gc:G12_Setting ,
                                                                                      gc:G13_Narrative_Location ,
                                                                                      gc:G14_Narrative-Stoff ,
                                                                                      gc:G1_Character ,
                                                                                      gc:G4_Social_Relationship ,
                                                                                      gc:G7_Fabula ,
                                                                                      gc:G8_Syuzhet ,
                                                                                      gc:G9_Narrative_Unit ;
                                                                     rdfs:comment "Also known as 'functional role'.A concept that classifies (in particular, it is 'played by') endurants, as used in some description. Roles are the descriptive counterpart of endurants, and, as endurants participate in perdurants, they usually have courses as modal targets (see).The typology of roles is still preliminary  ([DOLCE-Lite-Plus, 2005](https://www.w3.org/2001/sw/BestPractices/WNET/DLP3941_daml.html))."@en ;
                                                                     rdfs:label "role"@en .


###  http://www.ontologydesignpatterns.org/ont/dlp/ExtendedDnS.owl#situation
<http://www.ontologydesignpatterns.org/ont/dlp/ExtendedDnS.owl#situation> rdf:type owl:Class ;
                                                                          owl:disjointWith gc:G10_Narrative_Function ,
                                                                                           gc:G11_Narrative_Role ,
                                                                                           gc:G13_Narrative_Location ,
                                                                                           gc:G14_Narrative-Stoff ,
                                                                                           gc:G4_Social_Relationship ,
                                                                                           gc:G6_Relationship_Role ,
                                                                                           gc:G7_Fabula ,
                                                                                           gc:G8_Syuzhet ,
                                                                                           gc:G9_Narrative_Unit ;
                                                                          rdfs:comment "A situation is a social object that appears in the domain of an ontology only because there is a description whose components can 'carve up' a view (setting) on that domain. A situation has to satisfy a description (see below for ways of defining the satisfies relation), and it has to be setting for at least one entity.In other words, it is the ontological counterpart (with due local differences or restrictions) of settings (situations from SC, contexts, episodes, states of affairs, structures, configurations, cases, etc.).A perdurant is usually the only mandatory constituent of a setting.Two descriptions of a same situation are possible, otherwise we would result in a solipsistic ontology. The time and space (and possibly other qualities) of a situation are the time and space of the perdurants in the setting  ([DOLCE-Lite-Plus, 2005](https://www.w3.org/2001/sw/BestPractices/WNET/DLP3941_daml.html))." ;
                                                                          rdfs:label "situation" .


###  http://www.ontologydesignpatterns.org/ont/dlp/ExtendedDnS.owl#social-object
<http://www.ontologydesignpatterns.org/ont/dlp/ExtendedDnS.owl#social-object> rdf:type owl:Class ;
                                                                              rdfs:comment "A catch-all class for entities from the social world. It includes agentive and non-agentive socially-constructed objects: descriptions, concepts, figures, collections, information objects. It could be equivalent to 'non-physical object', but we leave the possibility open of 'private' non-physical objects  ([DOLCE-Lite-Plus, 2005](https://www.w3.org/2001/sw/BestPractices/WNET/DLP3941_daml.html))."@en ;
                                                                              rdfs:label "social object" .


###  http://www.w3.org/1999/02/22-rdf-syntax-ns#Seq
rdf:Seq rdf:type owl:Class ;
        rdfs:comment "The class of ordered containers."@en ;
        rdfs:isDefinedBy rdf: ;
        rdfs:label "Seq"@en .


###  https://ontology.golemlab.eu/G0_Character-Stoff
gc:G0_Character-Stoff rdf:type owl:Class ;
                      rdfs:subClassOf <http://www.cidoc-crm.org/cidoc-crm/E89_Propositional_Object> ,
                                      <http://www.ontologydesignpatterns.org/ont/dlp/ExtendedDnS.owl#social-object> ,
                                      [ rdf:type owl:Restriction ;
                                        owl:onProperty <http://www.cidoc-crm.org/cidoc-crm/P130i_features_are_also_found_on> ;
                                        owl:someValuesFrom gc:G1_Character
                                      ] ;
                      rdfs:comment "The concept of Character-Stoff is derived from the German term Erzählstoff, referring to narrative material (Zgoll et al, 2020). Character-Stoff represents the infinite potential of a character across all known and unknown variations, extending beyond any singular depiction. It encompasses all possible versions, features, actions, and roles of a character across time and media, while remaining open to reinterpretation and transformation. This polymorphous nature allows for endless modifications. Thus, Character-Stoff is an ever-evolving, inexhaustible phenomenon, impossible to outline in full."@en ;
                      rdfs:label "G0 Character-Stoff"@en ;
                      skos:example """Harry Potter. 
The Harry Potter Stoff includes not only the known versions from books, films, and fan works, but also potential reinterpretations in future media or cultural contexts. Any imaginary version of Harry Potter could be potentially true, as the Character-Stoff allows for infinite variations and reinterpretations.""" .


###  https://ontology.golemlab.eu/G10_Narrative_Function
gc:G10_Narrative_Function rdf:type owl:Class ;
                          rdfs:subClassOf <http://www.ontologydesignpatterns.org/ont/dlp/ExtendedDnS.owl#role> ,
                                          [ rdf:type owl:Restriction ;
                                            owl:onProperty <http://www.ontologydesignpatterns.org/ont/dlp/ExtendedDnS.owl#d-used-by> ;
                                            owl:someValuesFrom <http://iflastandards.info/ns/lrm/lrmoo/F1_Work>
                                          ] ,
                                          [ rdf:type owl:Restriction ;
                                            owl:onProperty <http://www.ontologydesignpatterns.org/ont/dlp/ExtendedDnS.owl#modal-target-of> ;
                                            owl:someValuesFrom gc:G7_Fabula
                                          ] ,
                                          [ rdf:type owl:Restriction ;
                                            owl:onProperty <http://www.ontologydesignpatterns.org/ont/dlp/ExtendedDnS.owl#modal-target-of> ;
                                            owl:someValuesFrom gc:G8_Syuzhet
                                          ] ,
                                          [ rdf:type owl:Restriction ;
                                            owl:onProperty <http://www.ontologydesignpatterns.org/ont/dlp/ExtendedDnS.owl#played-by> ;
                                            owl:someValuesFrom gc:G9_Narrative_Unit
                                          ] ;
                          owl:disjointWith gc:G12_Setting ,
                                           gc:G13_Narrative_Location ,
                                           gc:G14_Narrative-Stoff ,
                                           gc:G1_Character ,
                                           gc:G4_Social_Relationship ,
                                           gc:G7_Fabula ,
                                           gc:G8_Syuzhet ,
                                           gc:G9_Narrative_Unit ;
                          rdfs:comment "A narrative function refers to the functional roles that narrative units play within a story. For instance, the Proppian function (Propp, 1968) \"Villain causes harm or injury\" can be illustrated by the narrative unit where Zephyros causes Hyacinthus's death."@en ;
                          rdfs:label "G10 Narrative Function"@en ;
                          skos:example "Functions identified by Propp, Campbell, or Greimas (Greimas, 1983)." .


###  https://ontology.golemlab.eu/G11_Narrative_Role
gc:G11_Narrative_Role rdf:type owl:Class ;
                      rdfs:subClassOf <http://www.ontologydesignpatterns.org/ont/dlp/ExtendedDnS.owl#role> ,
                                      [ rdf:type owl:Restriction ;
                                        owl:onProperty <http://www.ontologydesignpatterns.org/ont/dlp/ExtendedDnS.owl#d-used-by> ;
                                        owl:someValuesFrom <http://iflastandards.info/ns/lrm/lrmoo/F1_Work>
                                      ] ,
                                      [ rdf:type owl:Restriction ;
                                        owl:onProperty <http://www.ontologydesignpatterns.org/ont/dlp/ExtendedDnS.owl#modal-target-of> ;
                                        owl:someValuesFrom gc:G7_Fabula
                                      ] ,
                                      [ rdf:type owl:Restriction ;
                                        owl:onProperty <http://www.ontologydesignpatterns.org/ont/dlp/ExtendedDnS.owl#modal-target-of> ;
                                        owl:someValuesFrom gc:G8_Syuzhet
                                      ] ,
                                      [ rdf:type owl:Restriction ;
                                        owl:onProperty <http://www.ontologydesignpatterns.org/ont/dlp/ExtendedDnS.owl#played-by> ;
                                        owl:someValuesFrom gc:G1_Character
                                      ] ;
                      owl:disjointWith gc:G12_Setting ,
                                       gc:G13_Narrative_Location ,
                                       gc:G14_Narrative-Stoff ,
                                       gc:G1_Character ,
                                       gc:G4_Social_Relationship ,
                                       gc:G7_Fabula ,
                                       gc:G8_Syuzhet ,
                                       gc:G9_Narrative_Unit ;
                      rdfs:comment "A narrative role refers to the functional roles that characters play within a story. Roles are only played by characters (gc:G1)." ;
                      rdfs:label "G11 Narrative Role" ;
                      skos:example "Narrator, dramatis personae from Propp Ontology (Pannach et al., 2021) or *commedia dell’arte*." .


###  https://ontology.golemlab.eu/G12_Setting
gc:G12_Setting rdf:type owl:Class ;
               rdfs:subClassOf <http://www.ontologydesignpatterns.org/ont/dlp/ExtendedDnS.owl#situation> ,
                               [ rdf:type owl:Restriction ;
                                 owl:onProperty <http://www.ontologydesignpatterns.org/ont/dlp/ExtendedDnS.owl#satisfies> ;
                                 owl:someValuesFrom <http://iflastandards.info/ns/lrm/lrmoo/F1_Work>
                               ] ,
                               [ rdf:type owl:Restriction ;
                                 owl:onProperty <http://www.ontologydesignpatterns.org/ont/dlp/ExtendedDnS.owl#setting-for> ;
                                 owl:someValuesFrom <http://www.ontologydesignpatterns.org/ont/dlp/DOLCE-Lite.owl#time-interval>
                               ] ,
                               [ rdf:type owl:Restriction ;
                                 owl:onProperty <http://www.ontologydesignpatterns.org/ont/dlp/ExtendedDnS.owl#setting-for> ;
                                 owl:someValuesFrom gc:G13_Narrative_Location
                               ] ,
                               [ rdf:type owl:Restriction ;
                                 owl:onProperty <http://www.ontologydesignpatterns.org/ont/dlp/ExtendedDnS.owl#setting-for> ;
                                 owl:someValuesFrom gc:G16_Object
                               ] ,
                               [ rdf:type owl:Restriction ;
                                 owl:onProperty <http://www.ontologydesignpatterns.org/ont/dlp/ExtendedDnS.owl#setting-for> ;
                                 owl:someValuesFrom gc:G1_Character
                               ] ,
                               [ rdf:type owl:Restriction ;
                                 owl:onProperty <http://www.ontologydesignpatterns.org/ont/dlp/ExtendedDnS.owl#setting-for> ;
                                 owl:someValuesFrom gc:G5_Narrative_Event
                               ] ;
               owl:disjointWith gc:G13_Narrative_Location ,
                                gc:G14_Narrative-Stoff ,
                                gc:G4_Social_Relationship ,
                                gc:G6_Relationship_Role ,
                                gc:G7_Fabula ,
                                gc:G8_Syuzhet ,
                                gc:G9_Narrative_Unit ;
               rdfs:comment "Setting is the narrative universe in which a story unfolds, encompassing the spatial, cultural, and social contexts that shape characters and events. It defines the situation and surroundings relevant to the narrative. Defining a setting for a Work is useful for its comparative and historical analysis with respect to other works. It is particularly apt to specify differences between canonical and fanfiction works that have Alternate Universe settings." ;
               rdfs:label "G12 Setting" ;
               skos:example """The Wizarding World for the Harry Potter novels. 
The “setting of “Eveline” [by J. Joyce] is early 20th-century lower-middle-class Dublin\" (Ryan, 2015).""" .


###  https://ontology.golemlab.eu/G13_Narrative_Location
gc:G13_Narrative_Location rdf:type owl:Class ;
                          rdfs:subClassOf <http://www.ontologydesignpatterns.org/ont/dlp/CommonSenseMapping.owl#non-physical-place> ,
                                          [ rdf:type owl:Restriction ;
                                            owl:onProperty <http://www.ontologydesignpatterns.org/ont/dlp/DOLCE-Lite.owl#generic-location-of> ;
                                            owl:someValuesFrom gc:G16_Object
                                          ] ,
                                          [ rdf:type owl:Restriction ;
                                            owl:onProperty <http://www.ontologydesignpatterns.org/ont/dlp/DOLCE-Lite.owl#generic-location-of> ;
                                            owl:someValuesFrom gc:G1_Character
                                          ] ,
                                          [ rdf:type owl:Restriction ;
                                            owl:onProperty <http://www.ontologydesignpatterns.org/ont/dlp/DOLCE-Lite.owl#generically-dependent-on> ;
                                            owl:someValuesFrom <http://www.loa-cnr.it/ontologies/CommonSenseMapping.owl#geographical-place>
                                          ] ,
                                          [ rdf:type owl:Restriction ;
                                            owl:onProperty <http://www.ontologydesignpatterns.org/ont/dlp/DOLCE-Lite.owl#proper-part> ;
                                            owl:someValuesFrom gc:G13_Narrative_Location
                                          ] ,
                                          [ rdf:type owl:Restriction ;
                                            owl:onProperty <http://www.ontologydesignpatterns.org/ont/dlp/DOLCE-Lite.owl#proper-part-of> ;
                                            owl:someValuesFrom gc:G13_Narrative_Location
                                          ] ,
                                          [ rdf:type owl:Restriction ;
                                            owl:onProperty <http://www.ontologydesignpatterns.org/ont/dlp/ExtendedDnS.owl#setting> ;
                                            owl:someValuesFrom gc:G12_Setting
                                          ] ,
                                          [ rdf:type owl:Restriction ;
                                            owl:onProperty <http://www.ontologydesignpatterns.org/ont/dlp/SpatialRelations.owl#participant-place-of> ;
                                            owl:someValuesFrom gc:G5_Narrative_Event
                                          ] ;
                          owl:disjointWith gc:G14_Narrative-Stoff ,
                                           gc:G4_Social_Relationship ,
                                           gc:G6_Relationship_Role ,
                                           gc:G7_Fabula ,
                                           gc:G8_Syuzhet ,
                                           gc:G9_Narrative_Unit ;
                          rdfs:comment "A narrative location is the spatial environment where events occur, the spatial frame that represents the immediate surroundings of action. It is a non-physical place shaped by the narrative context. A narrative location may derive features from real locations but it only exists as an entity within the narrative."@en ;
                          rdfs:label "G13 Narrative Location"@en ;
                          skos:example "England in the Harry Potter series functions as a non-physical place shaped by the narrative, generically dependent on England in the real world." .


###  https://ontology.golemlab.eu/G14_Narrative-Stoff
gc:G14_Narrative-Stoff rdf:type owl:Class ;
                       rdfs:subClassOf <http://www.cidoc-crm.org/cidoc-crm/E89_Propositional_Object> ,
                                       <http://www.ontologydesignpatterns.org/ont/dlp/ExtendedDnS.owl#description> ,
                                       [ rdf:type owl:Restriction ;
                                         owl:onProperty <http://www.cidoc-crm.org/cidoc-crm/P130i_features_are_also_found_on> ;
                                         owl:someValuesFrom gc:G7_Fabula
                                       ] ;
                       owl:disjointWith gc:G1_Character ,
                                        gc:G6_Relationship_Role ,
                                        gc:G7_Fabula ,
                                        gc:G8_Syuzhet ;
                       rdfs:comment "Narrative Stoff refers to the fundamental materials that form the basis of a narrative. It contains a chronological sequence of events (gc:G7_Fabula) that could be manifested across various narratives and media. This concept highlights the potential variations of narrative units within different contexts."@en ;
                       rdfs:label "G14 Narrative-Stoff"@en ;
                       skos:example "Apollo and Zephyros love Hyacinthus. While Apollo and Hyacinthus are playing a game with a discus, Zephyros uses the wind to change its direction, causing the discus to hit Hyacinthus and resulting in his death. Afterward, Hyacinthus transforms into a flower." .


###  https://ontology.golemlab.eu/G15_Fandom
gc:G15_Fandom rdf:type owl:Class ;
              rdfs:subClassOf <http://www.cidoc-crm.org/cidoc-crm/E28_Conceptual_Object> ,
                              <http://www.ontologydesignpatterns.org/ont/dlp/ExtendedDnS.owl#social-object> ,
                              [ rdf:type owl:Restriction ;
                                owl:onProperty <http://www.cidoc-crm.org/cidoc-crm/P130i_features_are_also_found_on> ;
                                owl:someValuesFrom <http://iflastandards.info/ns/lrm/lrmoo/F1_Work>
                              ] ;
              rdfs:comment "A fandom is a group of fans who share a common interest in a particular work or topic, such as a book or movie, and engage in fan activities like discussions or creating fan works."@en ;
              rdfs:label "G15 Fandom"@en ;
              skos:example "The entity identified by the label “Harry Potter - J. K. Rowling” on AO3." .


###  https://ontology.golemlab.eu/G16_Object
gc:G16_Object rdf:type owl:Class ;
              rdfs:subClassOf <http://www.cidoc-crm.org/cidoc-crm/E70_Thing> ,
                              <http://www.ontologydesignpatterns.org/ont/dlp/ExtendedDnS.owl#social-object> ,
                              [ rdf:type owl:Restriction ;
                                owl:onProperty <http://www.ontologydesignpatterns.org/ont/dlp/DOLCE-Lite.owl#generic-location> ;
                                owl:someValuesFrom gc:G13_Narrative_Location
                              ] ,
                              [ rdf:type owl:Restriction ;
                                owl:onProperty <http://www.ontologydesignpatterns.org/ont/dlp/ExtendedDnS.owl#setting> ;
                                owl:someValuesFrom gc:G12_Setting
                              ] ,
                              [ rdf:type owl:Restriction ;
                                owl:onProperty <http://www.ontologydesignpatterns.org/ont/dlp/ExtendedDnS.owl#used-by> ;
                                owl:someValuesFrom gc:G1_Character
                              ] ;
              rdfs:comment "An object refers to a persistent item that plays a significant role in the story but is not a character."@en ;
              rdfs:label "G16 Object"@en ;
              skos:example "The Elder Wand carried by Harry Potter." .


###  https://ontology.golemlab.eu/G17_Character_Feature
gc:G17_Character_Feature rdf:type owl:Class ;
                         rdfs:subClassOf gc:G2_Feature ;
                         rdfs:comment "Character traits or features are stable aspects defining a character's identity, including biographical (e.g., birth, death), physical (e.g., hair color, scars), and psychological features (e.g., personality). These three subcategories are specified using crm:E55_Type."@en ;
                         rdfs:label "G17 Character Feature"@en ;
                         skos:example """Harry Potter’s bravery as inferred from the sentence
“Harry screwed up his courage” (chapter 17 of Harry Potter and the Philosopher’s Stone).""" .


###  https://ontology.golemlab.eu/G18_Textual_Feature
gc:G18_Textual_Feature rdf:type owl:Class ;
                       rdfs:subClassOf gc:G2_Feature ;
                       rdfs:comment "Textual features are the elements or characteristics found in a narrative or fictions. These features include narrative style, like the tone and writing techniques employed by the author, as well as the point of view (POV) that determines the perspective from which the story is told, such as first-person or third-person. Textual features also contain the voice reflecting authors' attitude, the diction referring to the authors' choice of words, etc. Taxonomies of textual features can be further specified using crm:E55_Type." ;
                       rdfs:label "G18 Textual Feature" ;
                       skos:example "Stream of consciousness, first-person perspective" .


###  https://ontology.golemlab.eu/G1_Character
gc:G1_Character rdf:type owl:Class ;
                rdfs:subClassOf <http://www.cidoc-crm.org/cidoc-crm/E89_Propositional_Object> ,
                                <http://www.ontologydesignpatterns.org/ont/dlp/ExtendedDnS.owl#agentive-social-object> ,
                                [ rdf:type owl:Restriction ;
                                  owl:onProperty <http://www.cidoc-crm.org/cidoc-crm/P130_shows_features_of> ;
                                  owl:someValuesFrom gc:G0_Character-Stoff
                                ] ,
                                [ rdf:type owl:Restriction ;
                                  owl:onProperty <http://www.ontologydesignpatterns.org/ont/dlp/DOLCE-Lite.owl#participant-in> ;
                                  owl:someValuesFrom gc:G5_Narrative_Event
                                ] ,
                                [ rdf:type owl:Restriction ;
                                  owl:onProperty <http://www.ontologydesignpatterns.org/ont/dlp/ExtendedDnS.owl#involved-in> ;
                                  owl:someValuesFrom gc:G4_Social_Relationship
                                ] ,
                                [ rdf:type owl:Restriction ;
                                  owl:onProperty <http://www.ontologydesignpatterns.org/ont/dlp/ExtendedDnS.owl#plays> ;
                                  owl:someValuesFrom gc:G11_Narrative_Role
                                ] ,
                                [ rdf:type owl:Restriction ;
                                  owl:onProperty <http://www.ontologydesignpatterns.org/ont/dlp/ExtendedDnS.owl#plays> ;
                                  owl:someValuesFrom gc:G6_Relationship_Role
                                ] ,
                                [ rdf:type owl:Restriction ;
                                  owl:onProperty <http://www.ontologydesignpatterns.org/ont/dlp/ExtendedDnS.owl#setting> ;
                                  owl:someValuesFrom gc:G12_Setting
                                ] ,
                                [ rdf:type owl:Restriction ;
                                  owl:onProperty <http://www.ontologydesignpatterns.org/ont/dlp/ExtendedDnS.owl#uses> ;
                                  owl:someValuesFrom gc:G16_Object
                                ] ,
                                [ rdf:type owl:Restriction ;
                                  owl:onProperty gc:GP1_is_character_in ;
                                  owl:someValuesFrom <http://iflastandards.info/ns/lrm/lrmoo/F1_Work>
                                ] ;
                owl:disjointWith gc:G4_Social_Relationship ,
                                 gc:G6_Relationship_Role ,
                                 gc:G7_Fabula ,
                                 gc:G8_Syuzhet ,
                                 gc:G9_Narrative_Unit ;
                rdfs:comment "“Character is a text- or media-based figure in a storyworld, usually human or human-like,” understood through readers’ knowledge of real people (Jannidis, 2019). Readers attribute to characters mental states such as intentions and beliefs, and consider them to engage in actions. Characters can have specific functional roles within narratives, such as protagonist or antagonist, influencing how readers perceive and interpret the story."@en ;
                rdfs:label "G1 Character"@en ;
                skos:example "Harry Potter in the novel *Harry Potter and the Philosopher's Stone*." .


###  https://ontology.golemlab.eu/G2_Feature
gc:G2_Feature rdf:type owl:Class ;
              rdfs:subClassOf <http://www.cidoc-crm.org/cidoc-crm/E1_CRM_Entity> ;
              rdfs:comment """A feature in the context of narrative refers to a distinct element or characteristic that contributes to the structure and meaning of a story. Features include character traits and textual elements.
Taxonomies of features can be further specified using crm:E55_Type.""" ;
              rdfs:label "G2 Feature" ;
              skos:example "Style, theme, literary devices" .


###  https://ontology.golemlab.eu/G3_Psychological_State
gc:G3_Psychological_State rdf:type owl:Class ;
                          rdfs:subClassOf <http://www.ontologydesignpatterns.org/ont/dlp/DOLCE-Lite.owl#state> ,
                                          [ rdf:type owl:Restriction ;
                                            owl:onProperty <http://www.ontologydesignpatterns.org/ont/dlp/FunctionalParticipation.owl#state-of> ;
                                            owl:someValuesFrom gc:G1_Character
                                          ] ,
                                          [ rdf:type owl:Restriction ;
                                            owl:onProperty <http://www.ontologydesignpatterns.org/ont/dlp/TemporalRelations.owl#follows> ;
                                            owl:someValuesFrom gc:G3_Psychological_State
                                          ] ,
                                          [ rdf:type owl:Restriction ;
                                            owl:onProperty <http://www.ontologydesignpatterns.org/ont/dlp/TemporalRelations.owl#follows> ;
                                            owl:someValuesFrom gc:G5_Narrative_Event
                                          ] ,
                                          [ rdf:type owl:Restriction ;
                                            owl:onProperty <http://www.ontologydesignpatterns.org/ont/dlp/TemporalRelations.owl#precedes> ;
                                            owl:someValuesFrom gc:G3_Psychological_State
                                          ] ,
                                          [ rdf:type owl:Restriction ;
                                            owl:onProperty <http://www.ontologydesignpatterns.org/ont/dlp/TemporalRelations.owl#precedes> ;
                                            owl:someValuesFrom gc:G5_Narrative_Event
                                          ] ,
                                          [ rdf:type owl:Restriction ;
                                            owl:onProperty <http://www.ontologydesignpatterns.org/ont/dlp/TemporalRelations.owl#temporally-included-in> ;
                                            owl:someValuesFrom gc:G3_Psychological_State
                                          ] ,
                                          [ rdf:type owl:Restriction ;
                                            owl:onProperty <http://www.ontologydesignpatterns.org/ont/dlp/TemporalRelations.owl#temporally-included-in> ;
                                            owl:someValuesFrom gc:G5_Narrative_Event
                                          ] ,
                                          [ rdf:type owl:Restriction ;
                                            owl:onProperty <http://www.ontologydesignpatterns.org/ont/dlp/TemporalRelations.owl#temporally-includes> ;
                                            owl:someValuesFrom gc:G3_Psychological_State
                                          ] ,
                                          [ rdf:type owl:Restriction ;
                                            owl:onProperty <http://www.ontologydesignpatterns.org/ont/dlp/TemporalRelations.owl#temporally-includes> ;
                                            owl:someValuesFrom gc:G5_Narrative_Event
                                          ] ,
                                          [ rdf:type owl:Restriction ;
                                            owl:onProperty <http://www.ontologydesignpatterns.org/ont/dlp/TemporalRelations.owl#temporally-overlaps> ;
                                            owl:someValuesFrom gc:G3_Psychological_State
                                          ] ,
                                          [ rdf:type owl:Restriction ;
                                            owl:onProperty <http://www.ontologydesignpatterns.org/ont/dlp/TemporalRelations.owl#temporally-overlaps> ;
                                            owl:someValuesFrom gc:G5_Narrative_Event
                                          ] ;
                          rdfs:comment "A psychological state is a temporal mental condition that may change over time but possesses relatively constant qualities, such as emotions, motivations, beliefs, and goals."@en ;
                          rdfs:label "G3 Psychological State"@en ;
                          skos:example """Ron’s jealousy (Yule Ball).
In the Yule Ball scene, Ron’s jealousy stems from his unacknowledged feeling for Hermione and his insecurity. Seeing Hermione arriving at the ball with Viktor Krum, Ron lashes out and criticizes Hermione. His anger reveals his jealousy (chapter 23 of Harry Potter and The Goblet of Fire).""" .


###  https://ontology.golemlab.eu/G4_Social_Relationship
gc:G4_Social_Relationship rdf:type owl:Class ;
                          rdfs:subClassOf <http://www.loa-cnr.it/ontologies/ExtendedDnS.owl#social-relationship> ,
                                          [ rdf:type owl:Restriction ;
                                            owl:onProperty <http://www.ontologydesignpatterns.org/ont/dlp/DOLCE-Lite.owl#generically-dependent-on> ;
                                            owl:someValuesFrom gc:G5_Narrative_Event
                                          ] ,
                                          [ rdf:type owl:Restriction ;
                                            owl:onProperty <http://www.ontologydesignpatterns.org/ont/dlp/ExtendedDnS.owl#d-uses> ;
                                            owl:someValuesFrom gc:G6_Relationship_Role
                                          ] ,
                                          [ rdf:type owl:Restriction ;
                                            owl:onProperty <http://www.ontologydesignpatterns.org/ont/dlp/ExtendedDnS.owl#involves> ;
                                            owl:someValuesFrom gc:G1_Character
                                          ] ;
                          owl:disjointWith gc:G6_Relationship_Role ,
                                           gc:G7_Fabula ,
                                           gc:G8_Syuzhet ;
                          rdfs:comment "“A social description defining roles for the interaction of cognitive agents (DOLCE-Lite-Plus, 2005)” or dlp:agentive-social-objects. Characters are involved in social relationships."@en ;
                          rdfs:label "G4 Social Relationships"@en ;
                          skos:example """Romantic love between Ron and Hermione, which can be inferred from the paragraph below:
\"There was a clatter as the basilisk fangs cascaded out of Hermione’s arms. Running at Ron, she flung them around his neck and kissed him full on the mouth. Ron threw away the fangs and broomstick he was holding and responded with such enthusiasm that he lifted Hermione off her feet\" (chapter 31 in Harry Potter and the Deathly Hallows).""" .


###  https://ontology.golemlab.eu/G5_Narrative_Event
gc:G5_Narrative_Event rdf:type owl:Class ;
                      rdfs:subClassOf <http://www.ontologydesignpatterns.org/ont/dlp/DOLCE-Lite.owl#perdurant> ,
                                      [ rdf:type owl:Restriction ;
                                        owl:onProperty <http://www.ontologydesignpatterns.org/ont/dlp/DOLCE-Lite.owl#participant> ;
                                        owl:someValuesFrom gc:G1_Character
                                      ] ,
                                      [ rdf:type owl:Restriction ;
                                        owl:onProperty <http://www.ontologydesignpatterns.org/ont/dlp/ExtendedDnS.owl#setting> ;
                                        owl:someValuesFrom gc:G12_Setting
                                      ] ,
                                      [ rdf:type owl:Restriction ;
                                        owl:onProperty <http://www.ontologydesignpatterns.org/ont/dlp/SpatialRelations.owl#participant-place> ;
                                        owl:someValuesFrom gc:G13_Narrative_Location
                                      ] ,
                                      [ rdf:type owl:Restriction ;
                                        owl:onProperty <http://www.ontologydesignpatterns.org/ont/dlp/TemporalRelations.owl#follows> ;
                                        owl:someValuesFrom gc:G3_Psychological_State
                                      ] ,
                                      [ rdf:type owl:Restriction ;
                                        owl:onProperty <http://www.ontologydesignpatterns.org/ont/dlp/TemporalRelations.owl#follows> ;
                                        owl:someValuesFrom gc:G5_Narrative_Event
                                      ] ,
                                      [ rdf:type owl:Restriction ;
                                        owl:onProperty <http://www.ontologydesignpatterns.org/ont/dlp/TemporalRelations.owl#precedes> ;
                                        owl:someValuesFrom gc:G3_Psychological_State
                                      ] ,
                                      [ rdf:type owl:Restriction ;
                                        owl:onProperty <http://www.ontologydesignpatterns.org/ont/dlp/TemporalRelations.owl#precedes> ;
                                        owl:someValuesFrom gc:G5_Narrative_Event
                                      ] ,
                                      [ rdf:type owl:Restriction ;
                                        owl:onProperty <http://www.ontologydesignpatterns.org/ont/dlp/TemporalRelations.owl#temporally-included-in> ;
                                        owl:someValuesFrom gc:G3_Psychological_State
                                      ] ,
                                      [ rdf:type owl:Restriction ;
                                        owl:onProperty <http://www.ontologydesignpatterns.org/ont/dlp/TemporalRelations.owl#temporally-included-in> ;
                                        owl:someValuesFrom gc:G5_Narrative_Event
                                      ] ,
                                      [ rdf:type owl:Restriction ;
                                        owl:onProperty <http://www.ontologydesignpatterns.org/ont/dlp/TemporalRelations.owl#temporally-includes> ;
                                        owl:someValuesFrom gc:G3_Psychological_State
                                      ] ,
                                      [ rdf:type owl:Restriction ;
                                        owl:onProperty <http://www.ontologydesignpatterns.org/ont/dlp/TemporalRelations.owl#temporally-includes> ;
                                        owl:someValuesFrom gc:G5_Narrative_Event
                                      ] ,
                                      [ rdf:type owl:Restriction ;
                                        owl:onProperty <http://www.ontologydesignpatterns.org/ont/dlp/TemporalRelations.owl#temporally-overlaps> ;
                                        owl:someValuesFrom gc:G3_Psychological_State
                                      ] ,
                                      [ rdf:type owl:Restriction ;
                                        owl:onProperty <http://www.ontologydesignpatterns.org/ont/dlp/TemporalRelations.owl#temporally-overlaps> ;
                                        owl:someValuesFrom gc:G5_Narrative_Event
                                      ] ;
                      rdfs:comment "A narrative event is a unit inferred from a span of text and it can express a change of state, a process, or a state of things that supports the story, as defined by its temporality and sequentiality.. Events can be either external, like actions taken by characters, or psychological, involving changes in thoughts or feelings, which are distinct from a psychological state (cf. Gius and Vauth, 2022). Types of events can be specified using crm:E55_Type."@en ;
                      rdfs:label "G5 Narrative Event"@en ;
                      skos:example "\"There was a clatter as the basilisk fangs cascaded out of Hermione’s arms [process event]. Running at Ron [process event], she flung them around his neck and kissed him full on the mouth [change of state]. Ron threw away the fangs and broomstick [process event] he was holding and responded with such enthusiasm that he lifted Hermione off her feet [change of state].\"" .


###  https://ontology.golemlab.eu/G6_Relationship_Role
gc:G6_Relationship_Role rdf:type owl:Class ;
                        rdfs:subClassOf <http://www.ontologydesignpatterns.org/ont/dlp/ExtendedDnS.owl#role> ,
                                        [ rdf:type owl:Restriction ;
                                          owl:onProperty <http://www.ontologydesignpatterns.org/ont/dlp/ExtendedDnS.owl#d-used-by> ;
                                          owl:someValuesFrom gc:G4_Social_Relationship
                                        ] ,
                                        [ rdf:type owl:Restriction ;
                                          owl:onProperty <http://www.ontologydesignpatterns.org/ont/dlp/ExtendedDnS.owl#played-by> ;
                                          owl:someValuesFrom gc:G1_Character
                                        ] ;
                        owl:disjointWith gc:G7_Fabula ,
                                         gc:G8_Syuzhet ,
                                         gc:G9_Narrative_Unit ;
                        rdfs:comment "A relationship role refers to the functional role a character plays within the context of their interactions with other characters, serving as a descriptive counterpart to their enduring qualities, with characters participating in events (perdurants)." ;
                        rdfs:label "G6 Relationship Role" ;
                        skos:example """Lover (both Ron and Hermione in the “Ron and Hermione” romantic relationship).
Beloved (both Ron and Hermione in the “Ron and Hermione” romantic relationship).""" .


###  https://ontology.golemlab.eu/G7_Fabula
gc:G7_Fabula rdf:type owl:Class ;
             rdfs:subClassOf <http://www.ontologydesignpatterns.org/ont/dlp/ExtendedDnS.owl#course> ,
                             rdf:Seq ,
                             [ rdf:type owl:Restriction ;
                               owl:onProperty <http://www.cidoc-crm.org/cidoc-crm/P130_shows_features_of> ;
                               owl:someValuesFrom gc:G14_Narrative-Stoff
                             ] ,
                             [ rdf:type owl:Restriction ;
                               owl:onProperty <http://www.ontologydesignpatterns.org/ont/dlp/ExtendedDnS.owl#d-used-by> ;
                               owl:someValuesFrom <http://iflastandards.info/ns/lrm/lrmoo/F1_Work>
                             ] ,
                             [ rdf:type owl:Restriction ;
                               owl:onProperty <http://www.ontologydesignpatterns.org/ont/dlp/ExtendedDnS.owl#modal-target> ;
                               owl:someValuesFrom gc:G10_Narrative_Function
                             ] ,
                             [ rdf:type owl:Restriction ;
                               owl:onProperty <http://www.ontologydesignpatterns.org/ont/dlp/ExtendedDnS.owl#modal-target> ;
                               owl:someValuesFrom gc:G11_Narrative_Role
                             ] ,
                             [ rdf:type owl:Restriction ;
                               owl:onProperty <http://www.ontologydesignpatterns.org/ont/dlp/ExtendedDnS.owl#sequences> ;
                               owl:someValuesFrom gc:G5_Narrative_Event
                             ] ,
                             [ rdf:type owl:Restriction ;
                               owl:onProperty rdfs:member ;
                               owl:someValuesFrom gc:G9_Narrative_Unit
                             ] ;
             owl:disjointWith gc:G9_Narrative_Unit ;
             rdfs:comment "Fabula refers to the sequence of events of a narrative in chronological and causal order (Abbott, 2019). It represents the underlying structure of the story or what happens in it. Since the concept of fabula is mainly defined in relation to that of syuzhet, its conceptual function is to express a specific ordering of some narrative units. Accordingly, the fabula is a sequence (rdf:Seq) of narrative units (gc:G9) that orders (dlp:sequences) a set of temporal entities called events (dlp: perdurant)."@en ;
             rdfs:label "G7 Fabula"@en ;
             skos:example """Text: “1) I used to love this boy, and (2) he used to love me. (3) But I failed, he has been dead for years, and I am a god…(4) We were in a sunny field playing, as we both loved sports. He grabbed a diskus...He ran laughing to catch it. He should have gotten it, but in those last moments it felt like years....(5) A slight change in the wind destroyed everything. Instead of catching the diskus,it hit his head... I tried everything. Everything. Magic, all forms of healing. (6) But I could not bring him back. Me, the god of healing, failed…(7) and in its place a flower, more beautiful than royal phonecian, was born…(8) I dared Zephyros, the West Wind, who also loved Hyacinthus. I dared him to take him away from me. My greed caused his death” (fanfiction story [Smile as Bright as the Sun as You Fade into Darkness](https://archiveofourown.org/works/38717322/chapters/96804426) from AO3).

Fabula (sequence of hylemes, a type of G9_Narrative_Unit): 
H1: [Apollo] loves [Hyacinthus] (durative-constant)
H2: Zephyros loves Hyacinthus (durative-constant)
H3: [Hyacinthus] loves [Apollo] (durative-initial)
H4: [Apollo and Hyacinthus] play the game of discus (single-event)
H5: Zephyros is the West Wind. (durative-constant)
[H6: Zephyros causes the wind to change. (single-event)]
H7: The discus hits Hyacinthus (single-event)
H8: Apollo fails to save Hyacinthus (single-event)
H9: [Hyacinthus] is dead (durative-resultative)
[H10: Hyacinthus is a flower (durative-resultative)]""" .


###  https://ontology.golemlab.eu/G8_Syuzhet
gc:G8_Syuzhet rdf:type owl:Class ;
              rdfs:subClassOf <http://www.ontologydesignpatterns.org/ont/dlp/ExtendedDnS.owl#course> ,
                              rdf:Seq ,
                              [ rdf:type owl:Restriction ;
                                owl:onProperty <http://www.ontologydesignpatterns.org/ont/dlp/ExtendedDnS.owl#d-used-by> ;
                                owl:someValuesFrom <http://iflastandards.info/ns/lrm/lrmoo/F1_Work>
                              ] ,
                              [ rdf:type owl:Restriction ;
                                owl:onProperty <http://www.ontologydesignpatterns.org/ont/dlp/ExtendedDnS.owl#modal-target> ;
                                owl:someValuesFrom gc:G10_Narrative_Function
                              ] ,
                              [ rdf:type owl:Restriction ;
                                owl:onProperty <http://www.ontologydesignpatterns.org/ont/dlp/ExtendedDnS.owl#modal-target> ;
                                owl:someValuesFrom gc:G11_Narrative_Role
                              ] ,
                              [ rdf:type owl:Restriction ;
                                owl:onProperty <http://www.ontologydesignpatterns.org/ont/dlp/ExtendedDnS.owl#sequences> ;
                                owl:someValuesFrom gc:G5_Narrative_Event
                              ] ,
                              [ rdf:type owl:Restriction ;
                                owl:onProperty rdfs:member ;
                                owl:someValuesFrom gc:G9_Narrative_Unit
                              ] ;
              owl:disjointWith gc:G9_Narrative_Unit ;
              rdfs:comment "Often translated as \"plot\" or “discourse”, syuzhet encompasses how events are presented and organized within a narrative (Kukkonen, 2019; Abbott, 2019). It involves the specific ordering and techniques used to articulate the story, reflecting the author’s design and organization to achieve particular aesthetic and cognitive-emotional effects, like suspense.  As for fabula, the conceptual function of syuzhet is to express a specific ordering of some narrative units. Accordingly, the syuzhet is a sequence (rdf:Seq) of narrative units (gc:G9) that orders (dlp:sequences) a set of temporal entities called events (dlp: perdurant)."@en ;
              rdfs:label "G8 Syuzhet"@en ;
              skos:example """Text: “1) I used to love this boy, and (2) he used to love me. (3) But I failed, he has been dead for years, and I am a god…(4) We were in a sunny field playing, as we both loved sports. He grabbed a diskus...He ran laughing to catch it. He should have gotten it, but in those last moments it felt like years....(5) A slight change in the wind destroyed everything. Instead of catching the diskus,it hit his head... I tried everything. Everything. Magic, all forms of healing. (6) But I could not bring him back. Me, the god of healing, failed…(7) and in its place a flower, more beautiful than royal phonecian, was born…(8) I dared Zephyros, the West Wind, who also loved Hyacinthus. I dared him to take him away from me. My greed caused his death.” (fanfiction story [Smile as Bright as the Sun as You Fade into Darkness](https://archiveofourown.org/works/38717322/chapters/96804426) from AO3).

Syuthet (sequence of hylemes, a type of G9_Narrative_Unit): 
H4: [Apollo and Hyacinthus] play the game of discus (single-event)
H6: Zephyros causes the wind to change. (single-event)
H7: The discus hits Hyacinthus (single-event)
H8: Apollo fails to save Hyacinthus (single-event)
H9: [Hyacinthus] is dead (durative-resultative)
H10: Hyacinthus is a flower (durative-resultative)
H1: [Apollo] loves [Hyacinthus] (durative-constant)
H3: [Hyacinthus] loves [Apollo] (durative-initial)
H2: Zephyros loves Hyacinthus (durative-constant)
H5: Zephyros is the West Wind. (durative-constant)""" .


###  https://ontology.golemlab.eu/G9_Narrative_Unit
gc:G9_Narrative_Unit rdf:type owl:Class ;
                     rdfs:subClassOf <http://www.cidoc-crm.org/cidoc-crm/E89_Propositional_Object> ,
                                     <http://www.ontologydesignpatterns.org/ont/dlp/ExtendedDnS.owl#description> ,
                                     [ rdf:type owl:Restriction ;
                                       owl:onProperty <http://www.cidoc-crm.org/cidoc-crm/P67_refers_to> ;
                                       owl:someValuesFrom gc:G5_Narrative_Event
                                     ] ,
                                     [ rdf:type owl:Restriction ;
                                       owl:onProperty <http://www.ontologydesignpatterns.org/ont/dlp/DOLCE-Lite.owl#proper-part-of> ;
                                       owl:someValuesFrom <http://iflastandards.info/ns/lrm/lrmoo/F1_Work>
                                     ] ,
                                     [ rdf:type owl:Restriction ;
                                       owl:onProperty <http://www.ontologydesignpatterns.org/ont/dlp/ExtendedDnS.owl#plays> ;
                                       owl:someValuesFrom gc:G10_Narrative_Function
                                     ] ;
                     rdfs:comment "A narrative unit is the minimal or fundamental component of narrative structure that articulates actions, states, or thematic elements within a story. The advantage of having narrative unit as a concept distinct from that of narrative event (G5) is that narrative units can be propositional objects formulated differently from how events are presented in the narrative. For example, hylemes (Zgoll et al., 2023; Pannach, 2023) are narrative units (statements) composed of a subject, predicate, and optional object. They represent the fundamental building blocks of any narrative structure, describing actions, states, or information present within a narrative , such as \"Apollo loves Hyacinthus.\""@en ;
                     rdfs:label "G9 Narrative Unit"@en ;
                     skos:example "A hyleme." .


#################################################################
#    Annotations
#################################################################

<http://www.loa-cnr.it/ontologies/CommonSenseMapping.owl#collection-role> rdfs:comment "A role only played by collections." .


<http://www.loa-cnr.it/ontologies/ExtendedDnS.owl#flux> rdfs:comment "Fluxes are processes that (also) contain accomplishments as constituents. In other words, fluxes emerge out of accomplishments." .


<http://www.loa-cnr.it/ontologies/ExtendedDnS.owl#life-cycle> rdfs:comment "The course of events typical of the life of an object (kind)." .


<http://www.loa-cnr.it/ontologies/ExtendedDnS.owl#rational-physical-object> rdfs:comment "In this ontology, a rational object is encoded as having the ability to internally represent meta-descriptions (descriptions that have other descriptions playing roles used by them). Other theories of rational agency assume desires and intentions for these objects, but in principle any agent can have desires and intentions: the very difference seems to be the ability to choose among different desires or intentions by going 'meta-level'." .


<http://www.loa-cnr.it/ontologies/ExtendedDnS.owl#reconstructed-flux> rdfs:comment "Reconstructed fluxes are fluxes that only contain accomplishments as members." .


rdf:direction rdfs:comment "The base direction component of a CompoundLiteral." ;
              rdfs:isDefinedBy rdf: ;
              rdfs:label "direction" ;
              rdfs:seeAlso <https://www.w3.org/TR/json-ld11/#the-rdf-compoundliteral-class-and-the-rdf-language-and-rdf-direction-properties> .


rdf:language rdfs:comment "The language component of a CompoundLiteral." ;
             rdfs:isDefinedBy rdf: ;
             rdfs:label "language" ;
             rdfs:seeAlso <https://www.w3.org/TR/json-ld11/#the-rdf-compoundliteral-class-and-the-rdf-language-and-rdf-direction-properties> .


rdf:nil rdfs:comment "The empty list, with no items in it. If the rest of a list is nil then the list has no more items in it." ;
        rdfs:isDefinedBy rdf: ;
        rdfs:label "nil" .


###  Generated by the OWL API (version 4.5.26.2023-07-17T20:34:13Z) https://github.com/owlcs/owlapi
